before change refinement

new_proof/AuxTyping.v
@@ -8,6 +8,7 @@ From CT Require Import Refinement.
 From CT Require Import RefinementDenotation.
 From CT Require Import RefinementDenotationTac.
 From CT Require Import RefinementDenotationProp.
+From CT Require Import RDInv.
 
 Import Atom.
 Import CoreLang.
@@ -18,32 +19,28 @@ Import OperationalSemantics.
 Import OperationalSemanticsProp.
 Import BasicTyping.
 Import SyntaxSugar.
+Import TermOrdering.
 Import Refinement.
+Import RefinementTac.
 Import RefinementDenotation.
 Import RefinementDenotationTac.
 Import RefinementDenotationProp.
-
-Lemma wf_ctxrR_implies_ok: forall Γ, wf_ctxrR ∅ Γ -> ok Γ.
-Proof.
-  induction Γ; intros; auto.
-  invclear H; refinement_solver7.
-Qed.
-
-Global Hint Resolve wf_ctxrR_implies_ok: core.
+Import RDInv.
 
 Definition wf (Γ: listctx rty) (τ: rty) :=
-  wf_ctxrR_not_terr ∅ Γ /\ closed_rty 0 (ctxdom Γ) τ /\ not_overbasety τ.
+  wf_ctxrR_not_terr ∅ Γ /\ closed_rty 0 (ctxdom ⦑Γ⦒ ) τ /\ not_overbasety τ.
 
 Notation " Γ '⊢WF' τ " := (wf Γ τ) (at level 20, τ constr, Γ constr).
 
 Lemma well_formed_regular: forall Γ τ,
-  Γ ⊢WF τ -> wf_ctxrR ∅ Γ /\ closed_rty 0 (ctxdom Γ) τ /\ not_overbasety τ.
+  Γ ⊢WF τ -> wf_ctxrR ∅ Γ /\ closed_rty 0 (ctxdom ⦑Γ⦒ ) τ /\ not_overbasety τ.
 Proof.
   intros. destruct H. setoid_rewrite wf_ctxrR_iff_wf_ctxrR_not_terr.
   split; auto.
 Qed.
 
-Definition disjunction (Γ: listctx rty) (τ1 τ2 τ3: rty) := forall e, (⟦ τ1 ⟧{ Γ } e) /\ (⟦ τ2 ⟧{ Γ } e) <-> (⟦ τ3 ⟧{ Γ } e).
+Definition disjunction (Γ: listctx rty) (τ1 τ2 τ3: rty) :=
+  forall e, (⅋{∅}⟦ τ1 ⟧{ Γ } e) /\ (⅋{∅}⟦ τ2 ⟧{ Γ } e) <-> (⅋{∅}⟦ τ3 ⟧{ Γ } e).
 
 Notation " Γ '⊢' τ1 '⩔' τ2 '⩵' τ3 " := (disjunction Γ τ1 τ2 τ3) (at level 20, τ1 constr, τ2 constr, τ3 constr, Γ constr).
 
@@ -70,7 +67,7 @@ Proof.
   intros Γ τ1 τ2 H; induction H; split; intros; auto.
 Qed.
 
-Definition subtyping_spec: forall Γ τ1 τ2, wf_ctxrR ∅ Γ -> Γ ⊢ τ1 ⪡ τ2 -> (forall e, ⟦ τ1 ⟧{ Γ } e -> ⟦ τ2 ⟧{ Γ } e).
+Definition subtyping_spec: forall Γ τ1 τ2, wf_ctxrR ∅ Γ -> Γ ⊢ τ1 ⪡ τ2 -> (forall e, {∅}⟦ τ1 ⟧{ Γ } e -> {∅}⟦ τ2 ⟧{ Γ } e).
 Admitted.
 
 Reserved Notation "Γ '⊢' τ '⋮t' T" (at level 20).
@@ -82,14 +79,18 @@ Inductive term_under_type_check : listctx rty -> tm -> rty -> Prop :=
 | UT_Sub: forall Γ e (τ1 τ2:rty), Γ ⊢WF τ2 -> [] ⊢ e ⋮t τ1 -> [] ⊢ τ1 ⪡ τ2 ->  (Γ ⊢ e ⋮t τ2)
 | UT_Eq: forall Γ e τ1 τ2, Γ ⊢WF τ2 -> Γ ⊢ e ⋮t τ1 -> Γ ⊢ τ1 ⪡ τ2 -> Γ ⊢ τ2 ⪡ τ1 -> Γ ⊢ e ⋮t τ2
 | UT_Merge: forall Γ e (τ1 τ2 τ3: rty), Γ ⊢WF τ3 -> Γ ⊢ e ⋮t τ1 -> Γ ⊢ e ⋮t τ2 -> Γ ⊢ τ1 ⩔ τ2 ⩵ τ3 -> Γ ⊢ e ⋮t τ3
-| UT_Lete: forall Γ e_x e τ τ_x (L: aset),
+| UT_Lete_base: forall Γ e_x e τ b n d ϕ (L: aset),
+    Γ ⊢WF τ -> Γ ⊢ e_x ⋮t [v:b|n|d|ϕ] ->
+    (forall x, x ∉ L -> (Γ ++ [(x, [v:b|n|d|ϕ])]) ⊢ (e ^t^ x) ⋮t τ ) -> Γ ⊢ (tlete e_x e) ⋮t τ
+| UT_Lete_arr: forall Γ (e_x: value) e τ τ_x (L: aset),
+    is_arr τ_x ->
     Γ ⊢WF τ -> Γ ⊢ e_x ⋮t τ_x -> (forall x, x ∉ L -> (Γ ++ [(x, τ_x)]) ⊢ (e ^t^ x) ⋮t τ ) -> Γ ⊢ (tlete e_x e) ⋮t τ
 (* operators only take nat type *)
 | UT_LetOp: forall (Γ: listctx rty) op (v1 v2: value) e τ d1 d2 ϕ1 ϕ2 (L: aset),
     Γ ⊢WF τ ->
     Γ ⊢ v1 ⋮v [v: fst_ty_of_op op | 0 | d1 | ϕ1 ] ->
     Γ ⊢ v2 ⋮v [v: snd_ty_of_op op | 0 | d2 | ϕ2 ] ->
-    (forall x, x ∉ L -> (Γ ++ [(x, ((mk_op_ret op) ^r^ v1) ^r^ v2)]) ⊢ (e ^t^ x) ⋮t τ) ->
+    (forall x, x ∉ L -> (Γ ++ [(x, ({1 ~r> v2} ({0 ~r> v1} (mk_op_ret op))))]) ⊢ (e ^t^ x) ⋮t τ) ->
     Γ ⊢ (tletbiop op v1 v2 e) ⋮t τ
 | UT_LetAppIndepend: forall Γ (v1 v2: value) e τ τ2 τ_x (L: aset),
     Γ ⊢WF τ -> Γ ⊢ v1 ⋮v (τ2 ⤑ τ_x) -> Γ ⊢ v2 ⋮v τ2 -> (forall x, x ∉ L -> (Γ ++ [(x, τ_x)]) ⊢ (e ^t^ x) ⋮t τ) ->
@@ -126,93 +127,118 @@ where
 Scheme value_under_type_check_rec := Induction for value_under_type_check Sort Prop
     with term_under_type_check_rec := Induction for term_under_type_check Sort Prop.
 
-(* Lemma rRctx_backward_over: forall Γ z b n d ϕ (e: tm) τ, *)
-(*     ⟦ τ ⟧{ Γ ++ [(z, {v: b | n | d | ϕ})] } e <-> *)
-(*     (forall (u: value), ⟦ {v: b | n | d | ϕ} ⟧{ Γ } u -> ⟦ { z := u }r τ ⟧{ Γ } ({ z := u }t e)). *)
-(* Admitted. *)
-
-(* Lemma rRctx_backward_under: forall Γ z τ_z (e: tm) τ, *)
-(*     ~ not_overbasety τ_z -> *)
-(*     ⟦ τ ⟧{ Γ ++ [(z, τ_z)] } e <-> *)
-(*       (∃ (u_hat: tm), ⟦ τ_z ⟧{ Γ } u_hat /\ *)
-(*                         (forall (u: tm), ⟦ τ_z ⟧{ Γ } u -> *)
-(*                                     (∀ (v_u: value), u_hat ↪* v_u -> ⟦ { z:= v_u }r τ ⟧{ Γ } (tlete u (e ^t^ z))) *)
-(*                         )). *)
-(* Admitted. *)
-
 Ltac soundness_simp :=
   match goal with
   | [H: _ ⊢WF _ |- _ ] => apply well_formed_regular in H; mydestr
   end.
 
-Lemma mk_eq_constant_is_not_overbasety: forall c, not_overbasety (mk_eq_constant c).
+Lemma ok_dctx_weaken: forall Γ1 Γ2 d, ok_dctx d (Γ1 ++ Γ2) -> ok_dctx d Γ1.
 Proof.
-  intros. destruct c; simpl; auto.
+  induction Γ1; simpl; intros; mydestr; auto.
+  invclear H.
+  - constructor; eauto; listctx_set_simpl; try fast_set_solver.
+  - apply ok_dctx_cons_arr; eauto; listctx_set_simpl; try fast_set_solver.
 Qed.
 
-Global Hint Resolve mk_eq_constant_is_not_overbasety: core.
-
-Lemma mk_eq_var_is_not_overbasety: forall b x, not_overbasety (mk_eq_var b x).
+Lemma wf_ctxrR_weaken: forall Γ1 Γ2 st, wf_ctxrR st (Γ1 ++ Γ2) -> wf_ctxrR st Γ1.
 Proof.
-  intros. destruct b; simpl; auto.
+  induction Γ1; simpl; intros; mydestr; auto. constructor.
+  invclear H. invclear H3; auto_ty_exfalso.
+  - constructor; eauto. apply ok_dctx_weaken with (Γ2:=Γ2). listctx_set_simpl.
+  - mydestr. constructor; eauto. apply ok_dctx_weaken with (Γ2:=Γ2). listctx_set_simpl.
+  - constructor; eauto. apply ok_dctx_weaken with (Γ2:=Γ2). listctx_set_simpl.
 Qed.
 
-Global Hint Resolve mk_eq_var_is_not_overbasety: core.
-
-Lemma is_arr_implies_not_overbasety: forall τ, is_arr τ -> not_overbasety τ.
+Lemma wf_ctxrR_implies_inner_closed_rty: forall Γ1 x τ_x Γ2 st,
+    wf_ctxrR st (Γ1 ++ (x, τ_x) :: Γ2) -> closed_rty 0 (ctxdom ⦑Γ1⦒ ∪ dom aset st) τ_x.
 Proof.
-  intros. destruct τ; simpl; auto; invclear H; auto.
+  induction Γ1; simpl; intros; mydestr; auto.
+  - invclear H; refinement_solver.
+    + invclear H3; refinement_solver.
+    + invclear H5; refinement_solver.
+  - invclear H; refinement_solver.
+    + apply ok_dctx_regular2 in H3; mydestr.
+      assert ((a, {v:B|n|d|ϕ}) :: Γ1 ++ (x, τ_x) :: Γ2 = ((a, {v:B|n|d|ϕ}) :: Γ1) ++ [(x, τ_x)] ++ Γ2) as Hz by listctx_set_simpl.
+      apply H in Hz. inv_rd_simpl0.
+    + apply ok_dctx_regular2 in H4; mydestr.
+      assert ((a, [v:B|n|d|ϕ]) :: Γ1 ++ (x, τ_x) :: Γ2 = ((a, [v:B|n|d|ϕ]) :: Γ1) ++ [(x, τ_x)] ++ Γ2) as Hz by listctx_set_simpl.
+      apply H1 in Hz. inv_rd_simpl0.
+    + apply ok_dctx_regular2 in H5; mydestr.
+      assert ((a, r) :: Γ1 ++ (x, τ_x) :: Γ2 = ((a, r) :: Γ1) ++ [(x, τ_x)] ++ Γ2) as Hz by listctx_set_simpl.
+      apply H in Hz. dec_solver2. inv_rd_simpl0.
 Qed.
 
-Global Hint Resolve is_arr_implies_not_overbasety: core.
-
-(* Theorem judge_implies_not_overbasety: *)
-(*   forall (Γ: listctx rty) (e: tm) (τ: rty), Γ ⊢ e ⋮t τ -> not_overbasety τ. *)
-(* Proof. *)
-(*   apply (term_under_type_check_rec *)
-(*            (fun Γ v τ _ => not_overbasety τ) *)
-(*            (fun Γ e τ _ => not_overbasety τ)); intros Γ; intros; mydestr; simpl; auto; *)
-(*     try match goal with *)
-(*     | [H: _ ⊢ ?τ1 ⪡ ?τ2 |- not_overbasety ?τ2] => *)
-(*         apply subtyping_implies_not_overbasety in H; rewrite <- H; auto *)
-(*     | [H: _ ⊢ ?τ1 ⪡ ?τ2 |- not_overbasety ?τ1] => *)
-(*         apply subtyping_implies_not_overbasety in H; rewrite H; auto *)
-(*     end. *)
-(*   - admit. *)
-(*   - auto_pose_fv x; repeat specialize_with x; auto. *)
-(*   - auto_pose_fv x; repeat specialize_with x; auto. *)
-(*   - auto_pose_fv x; repeat specialize_with x; auto. *)
-(*   - auto_pose_fv x; repeat specialize_with x; auto. *)
-(* Admitted. *)
-
-    (* rewrite rR_shadow_update_st in H11. admit. refinement_solver. *)
-    (* setoid_rewrite close_open_var_tm in H11. admit. refinement_solver. *)
-
-
-
-
-Theorem soundness: forall (Γ: listctx rty) (e: tm) (τ: rty), Γ ⊢ e ⋮t τ -> ⟦ τ ⟧{ Γ } e.
+Lemma rty_judgement_implies_wf: forall (Γ: listctx rty) e (τ: rty), Γ ⊢ e ⋮t τ -> Γ ⊢WF τ.
 Proof.
-  (* intros. assert (not_overbasety τ) by (eapply judge_implies_not_overbasety; eauto). *)
-  (* generalize dependent τ. generalize dependent e. generalize dependent Γ. *)
   apply (term_under_type_check_rec
-           (fun Γ v τ _ => ⟦ τ ⟧{ Γ } v)
-           (fun Γ e τ _ => ⟦ τ ⟧{ Γ } e)); intros Γ; intros; mydestr; try soundness_simp.
+           (fun Γ v τ _ => Γ ⊢WF τ)
+           (fun Γ e τ _ => Γ ⊢WF τ)); intros Γ; intros; mydestr; auto.
+Qed.
+
+Lemma inv_rRctx_tletbiop_all: forall Γ st (τ: rty) x op n1 d1 ϕ1 n2 d2 ϕ2 (v1 v2: value) e,
+    x ∉ fv_tm e -> x ∉ rty_fv τ -> not_overbasety τ ->
+    wf_ctxrR st (Γ ++ [(x, {1 ~r> v2} (mk_op_ret op ^r^ v1))]) ->
+    (⅋{st}⟦[v:fst_ty_of_op op|n1|d1|ϕ1]⟧{Γ}) v1 ->
+    (⅋{st}⟦[v:fst_ty_of_op op|n2|d2|ϕ2]⟧{Γ}) v2 ->
+    (⅋{st}⟦τ⟧{Γ ++ [(x, {1 ~r> v2} (mk_op_ret op ^r^ v1))] }) (e ^t^ x) ->
+    ⅋{st}⟦τ⟧{Γ ++ [(x, {1 ~r> v2} (mk_op_ret op ^r^ v1))] } (tletbiop op v1 v2 e).
+Proof.
+  induction Γ; intros; RD_simp2.
+  - mydestr. inv_rd_simpl1. constructor; auto.
+    + denotation_simp. assert ([] ⊢t tletbiop op v1 v2 e ⋮t ⌊τ⌋). eapply tletbiop_typable; refinement_solver.
+      basic_typing_solver.
+    + exists (eval_op_under_bound_tm op v1 v2). split. apply rR_eval_op_under_bound_tm.
+      intros. assert (x1 ↪* v_x) as Hz by (eapply rR_eval_op_under_bound_tm_min; eauto).
+      auto_under v_x. RD_simp2. simpl.
+      rewrite subst_fresh_tm; auto. rewrite open_subst_same_tm in H10; auto.
+      eapply termR_perserve_rR; refinement_solver.
+      eapply letapp_eval_op_under_bound_tm_termR; eauto; refinement_solver.
+  - constructor; auto. denotation_simp. apply tletbiop_typable_ctx_dummy_cons; auto.
+    intros. auto_under c_x. simpl. eapply IHΓ; eauto.
+    + rewrite fv_of_subst_tm_closed; refinement_solver.
+    + rewrite <- subst_open_var_tm; auto. denotation_simp. basic_typing_solver.
+  - constructor; auto. denotation_simp. apply tletbiop_typable_ctx_dummy_cons; auto.
+    mydestr. auto_meet_exists Hmeet. auto_meet_reduce. auto_under v_x. eapply IHΓ; eauto; fold tm_subst.
+    + rewrite fv_of_subst_tm_closed; refinement_solver.
+    + rewrite <- subst_open_var_tm; auto. denotation_simp. basic_typing_solver. op_solver1.
+  - constructor; auto. denotation_simp. apply tletbiop_typable_ctx_dummy_cons; auto.
+    intros. auto_under v_x. eapply IHΓ; eauto; fold tm_subst.
+    + rewrite fv_of_subst_tm_closed; refinement_solver.
+    + rewrite <- subst_open_var_tm; auto. denotation_simp. basic_typing_solver. refinement_solver.
+Qed.
+
+Theorem soundness: forall (Γ: listctx rty) (e: tm) (τ: rty), Γ ⊢ e ⋮t τ -> ⅋{∅}⟦ τ ⟧{ Γ } e.
+Proof.
+  apply (term_under_type_check_rec
+           (fun Γ v τ _ => ⅋{∅}⟦ τ ⟧{ Γ } v)
+           (fun Γ e τ _ => ⅋{∅}⟦ τ ⟧{ Γ } e)); intros Γ; intros; mydestr; try soundness_simp.
   (* constant *)
-  - apply rRctx_pre_weakening_empty; auto. admit.
+  - apply inv_rRctx_pre_weakening_empty; auto. admit.
   (* var base *)
   - apply ctxfind_some_spec in H; auto; mydestr; subst.
-    rewrite app_assoc. apply rRctx_pre_weakening; refinement_solver.
-    admit.
+    rewrite app_assoc.
+    apply inv_rRctx_pre_weakening; refinement_solver.
+    apply wf_ctxrR_implies_inv_var_over_last.
+    eapply wf_ctxrR_weaken; listctx_set_simpl; eauto.
   - apply ctxfind_some_spec in H; auto; mydestr; subst.
-    rewrite app_assoc. apply rRctx_pre_weakening; refinement_solver.
-    admit.
+    rewrite app_assoc.
+    apply inv_rRctx_pre_weakening; refinement_solver.
+    apply wf_ctxrR_implies_inv_var_under_last.
+    eapply wf_ctxrR_weaken; listctx_set_simpl; eauto.
   (* var arr *)
   - apply ctxfind_some_spec in e; auto; mydestr; subst.
-    rewrite app_assoc. apply rRctx_pre_weakening; refinement_solver. admit.
+    rewrite app_assoc.
+    apply inv_rRctx_pre_weakening; refinement_solver.
+    apply wf_ctxrR_implies_inv_var_is_arr_last; auto.
+    eapply wf_ctxrR_implies_inner_closed_rty; eauto.
+    eapply wf_ctxrR_weaken; listctx_set_simpl; eauto.
   (* lam *)
-  - auto_pose_fv x. repeat specialize_with x. admit.
-  - auto_pose_fv x. repeat specialize_with x. admit.
+  - auto_pose_fv x. repeat specialize_with x.
+    eapply inv_rRctx_oarr; eauto; refinement_solver2.
+    apply rty_judgement_implies_wf in t; eauto. soundness_simp; auto.
+  - auto_pose_fv x. repeat specialize_with x.
+    eapply inv_rRctx_arrarr; eauto; refinement_solver2.
+    apply rty_judgement_implies_wf in t. soundness_simp; auto.
   (* fix *)
   - admit.
   (* value *)
@@ -220,22 +246,40 @@ Proof.
   (* err *)
   - admit.
   (* sub *)
-  - apply subtyping_spec with (e := e) in s; RD_simp; auto.
-    + apply rRctx_pre_weakening_empty; auto.
+  - apply subtyping_spec with (e := e) in s; RD_simp2; auto.
+    + RD_simp. apply inv_rRctx_pre_weakening_empty; auto.
     + constructor.
+    + constructor; auto.
   (* eq *)
-  - eapply subtyping_spec; eauto.
+  - admit.
   (* merge *)
   - match goal with
     | [H: _ ⊢ _ ⩔ _ ⩵ _ |- _ ] => unfold disjunction in H; erewrite <- H; split; auto
     end.
   (* lete *)
-  - auto_pose_fv x. repeat specialize_with x. admit.
+  - auto_pose_fv x. repeat specialize_with x. eapply wf_implies_ctxrR_tlete_ubase_drop in H0; eauto. setoid_rewrite close_open_var_tm in H0; fast_set_solver.
+    apply rty_judgement_implies_wf in t0. soundness_simp; auto.
+    refinement_solver.
+  - auto_pose_fv x. repeat specialize_with x. eapply wf_implies_ctxrR_tlete_is_arr_drop in H0; eauto. setoid_rewrite close_open_var_tm in H0; fast_set_solver.
+    apply rty_judgement_implies_wf in t0. soundness_simp; auto.
+    refinement_solver.
   (* letop *)
-  - auto_pose_fv x. repeat specialize_with x. admit.
+  - auto_pose_fv x. repeat specialize_with x.
+    apply inv_implies_ctxrR_drop_last with (x:=x) (τ_x:= ({1 ~r> v2} (mk_op_ret op ^r^ v1))); eauto; try fast_set_solver.
+    + apply rty_judgement_implies_wf in t. soundness_simp; auto.
+    + refinement_solver.
+    + assert (exists n1: nat, v1 = n1). eapply fst_ty_of_op_implies_nat; eauto.
+
+      Check inv_rRctx_tletbiop. eapply inv_rRctx_tletbiop.
+  - inv_rd_simpl1. assert (x ∉ ctxdom ⦑Γ⦒); ctx_erase_simp. set_solver.
+  - assert (x ∉ fv_tm e_x). inv_rd_solver1.
+    assert (x ∉ fv_tm (x \t\ e)) by apply close_rm_fv_tm.
+    set_solver.
+
+    admit.
   - auto_pose_fv x. repeat specialize_with x. admit.
   - auto_pose_fv x. repeat specialize_with x. admit.
   (* matchb true *)
-  - admit.
-  - admit.
+  - admit. (* easy *)
+  - admit. (* easy *)
 Admitted.
