new_proof/RefinementDenotationProp.v
@@ -31,21 +31,93 @@ Import TermOrdering.
 
 Inductive wf_ctxrR: state -> listctx rty -> Prop :=
 | wf_ctxrR_nil: forall st, wf_ctxrR st []
-| ctxrR_cons_over: forall st (x: atom) B n d ϕ Γ,
+| wf_ctxrR_cons_over: forall st (x: atom) B n d ϕ Γ,
     ok_dctx (dom _ st) ((x, {v: B | n | d | ϕ}) :: Γ) ->
     (* (exists (c_wf: constant), {st}⟦ {v: B | n | d | ϕ} ⟧ c_wf) -> *)
     (forall (c_x: constant), {st}⟦ {v: B | n | d | ϕ} ⟧ c_x ->
                         wf_ctxrR (<[ x := c_x ]> st) Γ) ->
     wf_ctxrR st ((x, {v: B | n | d | ϕ}) :: Γ)
-| ctxrR_cons_under: forall st (x: atom) τ_x Γ,
-    not_overbasety τ_x ->
-    ok_dctx (dom _ st) ((x, τ_x) :: Γ) ->
-    (forall e_wf, {st}⟦ τ_x ⟧ e_wf -> (exists (v_wf: value), e_wf ↪* v_wf)) ->
-    (exists e_x_hat, {st}⟦ τ_x ⟧ e_x_hat /\
-                  (forall e_x, {st}⟦ τ_x ⟧ e_x ->
+| wf_ctxrR_cons_under_base: forall st (x: atom) B n d ϕ Γ,
+    ok_dctx (dom _ st) ((x, [v: B | n | d | ϕ] ) :: Γ) ->
+    (forall e_wf, {st}⟦ [v: B | n | d | ϕ] ⟧ e_wf -> (exists (v_wf: value), e_wf ↪* v_wf)) ->
+    (exists e_x_hat, {st}⟦ [v: B | n | d | ϕ] ⟧ e_x_hat /\
+                  (forall e_x, {st}⟦ [v: B | n | d | ϕ] ⟧ e_x ->
                           (∀ (v_x: value), e_x_hat ↪* v_x ->
                                            wf_ctxrR ({ x ↦ v_x } st) Γ ))) ->
-     wf_ctxrR st ((x, τ_x) :: Γ).
+    wf_ctxrR st ((x, [v: B | n | d | ϕ]) :: Γ)
+| wf_ctxrR_cons_under_arr: forall st (x: atom) τ_x Γ,
+    is_arr τ_x ->
+    ok_dctx (dom _ st) ((x, τ_x) :: Γ) ->
+    (forall e_wf, {st}⟦ τ_x ⟧ e_wf -> (exists (v_wf: value), e_wf ↪* v_wf)) ->
+    wf_ctxrR st Γ ->
+    wf_ctxrR st ((x, τ_x) :: Γ).
+
+Ltac auto_meet_exists HE :=
+  match goal with
+  | [H1: ({0;b∅;?st}⟦[v:?b|?n|?d|?ϕ]⟧) ?x1,
+        H2: ({0;b∅;?st}⟦[v:?b|?n|?d|?ϕ]⟧) ?x2,
+          H3: ({0;b∅;?st}⟦[v:?b|?n|?d|?ϕ]⟧) ?x3 |- ∃ e, {0;b∅;?st}⟦[v:?b|?n|?d|?ϕ]⟧ e /\ _ ] =>
+      exists ((x1 ⊗{ b } x2) ⊗{ b } x3) ; assert ( {0;b∅;st}⟦[v:b|n|d|ϕ]⟧ ((x1 ⊗{ b } x2) ⊗{ b } x3)) as HE by (eapply rR_tmeet3_when_all; auto); split; auto; intros
+  | [H1: ({0;b∅;?st}⟦[v:?b|?n|?d|?ϕ]⟧) ?x1,
+        H2: ({0;b∅;?st}⟦[v:?b|?n|?d|?ϕ]⟧) ?x2 |- ∃ e, {0;b∅;?st}⟦[v:?b|?n|?d|?ϕ]⟧ e /\ _ ] =>
+      exists (x1 ⊗{ b } x2); assert ( {0;b∅;st}⟦[v:b|n|d|ϕ]⟧ (x1 ⊗{ b } x2)) as HE by (eapply rR_tmeet_when_both; eauto); split; auto; intros
+  | [H1: ({0;b∅;?st}⟦[v:?b|?n|?d|?ϕ]⟧) ?x1 |- ∃ e, {0;b∅;?st}⟦[v:?b|?n|?d|?ϕ]⟧ e /\ _ ] =>
+      exists x1; split; eauto; intros
+  | [|- ∃ e, {0;b∅;?st}⟦?r⟧ e /\ _ ] =>
+      assert ({0;b∅;st}⟦r⟧ (random_inhabitant r)) by (apply random_inhabitant_in_any_under; refinement_solver7);
+      eexists; split; eauto; intros
+  end.
+
+Ltac auto_meet_reduce :=
+  match goal with
+  | [H: ((?x1 ⊗{ ?b } ?x2) ⊗{ ?b } ?x3) ↪* ?v |- _ ] =>
+      rewrite reduction_tmeet3_iff_all in H; refinement_solver7; mydestr; eauto
+  | [H: (?x1 ⊗{ ?b} ?x2) ↪* ?v |- _ ] =>
+      rewrite reduction_tmeet_iff_both in H; refinement_solver7; mydestr; eauto
+  end.
+
+Ltac auto_under_specialize e :=
+  repeat (match goal with
+          | [He: ?P (tvalue e), H: forall e_x, ?P e_x -> _ |- _ ] => specialize (H _ He)
+          | [He: ?P e, H: forall e_x, ?P e_x -> _ |- _ ] => specialize (H _ He)
+          | [He: ?P (tvalue e), H: forall e_x, _ (tvalue e_x) -> _ |- _ ] => specialize (H _ He)
+          | [He: ?P (tvalue (vconst e)), H: forall c_x, _ (tvalue (vconst c_x)) -> _ |- _ ] => specialize (H _ He)
+          end; mydestr).
+
+Ltac auto_under_reduction_specialize :=
+  repeat match goal with
+    | [H: forall v, ?e ↪* (tvalue _) → _, H': ?e ↪* (tvalue _) |- _ ] => specialize (H  _ H')
+    (* | [H: forall v, ?e ↪* (tvalue _) → _, H': ?e ↪* (tvalue _) |- _ ] => specialize (H  _ H') *)
+    end.
+
+Ltac auto_under e :=
+  auto_under_specialize e; auto_under_reduction_specialize.
+
+Lemma is_arr_implies_random_inhabitant_is_value: forall τ_x, is_arr τ_x -> (exists (v: value), random_inhabitant τ_x = v).
+Proof.
+  induction τ_x; simpl; intro; invclear H; eauto.
+Qed.
+
+Lemma mk_eq_constant_is_not_overbasety: forall c, not_overbasety (mk_eq_constant c).
+Proof.
+  intros. destruct c; simpl; auto.
+Qed.
+
+Global Hint Resolve mk_eq_constant_is_not_overbasety: core.
+
+Lemma mk_eq_var_is_not_overbasety: forall b x, not_overbasety (mk_eq_var b x).
+Proof.
+  intros. destruct b; simpl; auto.
+Qed.
+
+Global Hint Resolve mk_eq_var_is_not_overbasety: core.
+
+Lemma is_arr_implies_not_overbasety: forall τ, is_arr τ -> not_overbasety τ.
+Proof.
+  intros. destruct τ; simpl; auto; invclear H; auto.
+Qed.
+
+Global Hint Resolve is_arr_implies_not_overbasety: core.
 
 Lemma wf_ctxrR_iff_wf_ctxrR_not_terr: forall (Γ: listctx rty) st, wf_ctxrR st Γ <-> wf_ctxrR_not_terr st Γ.
 Proof.
@@ -54,13 +126,24 @@ Proof.
   - constructor; auto.
   - invclear H.
     + constructor; auto. intros. rewrite <- IHΓ; auto.
-    + constructor; auto.
-      assert (valid_rty τ_x) as Hz by refinement_solver.
-      intro Hf. apply H5 in Hf. mydestr. reduction_simpl1.
+    + mydestr. constructor; auto. simpl; auto. intro Hf. apply H4 in Hf. mydestr. reduction_simpl1.
       mydestr. exists x0. split; auto.
       intros. rewrite <- IHΓ; eauto.
-  - invclear H.
-    + constructor; auto. intros. rewrite IHΓ; auto.
+    + constructor; auto.
+      intro Hf. apply H5 in Hf. mydestr. reduction_simpl1.
+      mydestr.
+      assert ({0;b∅;st}⟦τ_x⟧ (random_inhabitant τ_x)).
+      apply random_inhabitant_in_any_under; refinement_solver7.
+      eexists; split; eauto. intros. rewrite <- IHΓ; eauto. erewrite state_insert_closed_value_arr; eauto.
+      refinement_solver.
+  - invclear H. constructor; auto. intros. rewrite IHΓ; auto.
+    destruct (decide (is_arr τ_x)); auto_ty_exfalso.
+    + mydestr.
+      assert (∀ e_wf : tm, ({0;b∅;st}⟦τ_x⟧) e_wf → ∃ v_wf : value, e_wf ↪* v_wf) as Hv.
+      intros. eapply not_rR_inhabitant_err_implies_halt in H5; eauto; refinement_solver.
+      constructor; auto.
+      specialize (Hv _ H). mydestr. specialize (H0 _ H _ H1). rewrite <- IHΓ in H0.
+      erewrite state_insert_closed_value_arr in H0; eauto. refinement_solver.
     + constructor; auto.
       intros. eapply not_rR_inhabitant_err_implies_halt in H5; eauto; refinement_solver.
       mydestr. exists x0. split; auto.
@@ -68,6 +151,39 @@ Proof.
 Qed.
 
 Global Hint Constructors ok_dctx: core.
+
+Lemma rR_implies_no_free: forall st e τ a, ({0;b∅;st}⟦τ⟧) e -> a ∉ fv_tm e.
+Proof.
+  intros. refinement_solver7. basic_typing_solver7. set_solver.
+Qed.
+
+Global Hint Resolve rR_implies_no_free: core.
+
+Lemma ctxrR_tlete_drop_halt_lhs: forall st τ τ_x a e_x e,
+    not_overbasety τ ->
+   {0;b∅;st}⟦τ⟧ e -> {0;b∅;st}⟦τ_x⟧ e_x ->
+   (∃ v : value, e_x ↪* v) ->
+   ({0;b∅;st}⟦τ⟧) (tlete e_x (a \t\ e)).
+Proof.
+  intros.
+  eapply termR_perserve_rR; eauto; refinement_solver5.
+  eapply termR_tlete_drop_halt_lhs'; refinement_solver7.
+Qed.
+
+Global Hint Resolve ctxrR_tlete_drop_halt_lhs: core.
+
+(* Lemma rR_random_inhabitant: forall st r, {0;b∅;st}⟦r⟧ (random_inhabitant r). *)
+(* Proof. *)
+(*   intros. apply random_inhabitant_in_any_under; refinement_solver7. *)
+
+Lemma rR_implies_reduction_no_free: forall st r e (v: value),
+({0;b∅;st}⟦r⟧) e -> e ↪* v -> closed_value v.
+Proof.
+  intros.
+  assert ([] ⊢t v ⋮v ⌊ r ⌋);eauto. refinement_solver.
+Qed.
+
+Global Hint Resolve rR_implies_reduction_no_free: core.
 
 Lemma rRctx_pre_weakening_empty: forall Γ st τ,
     not_overbasety τ ->
@@ -78,26 +194,14 @@ Proof.
   invclear H0.
   - invclear H5; auto_ty_exfalso. constructor; refinement_solver7.
     intros. apply IHΓ; auto.
-    rewrite subst_fresh_tm.
+    rewrite subst_fresh_tm; eauto.
     rewrite rR_shadow_update_st_c; refinement_solver.
-    refinement_solver7. basic_typing_solver7. set_solver.
-  - destruct (decide (is_arr r)).
-    + apply ctxrR_cons_under_arr; refinement_solver7. mydestr.
-      exists x; split; auto. intros. apply IHΓ; eauto.
-      rewrite rR_shadow_update_st; refinement_solver.
-      eapply termR_perserve_rR; eauto; refinement_solver5.
-      eapply termR_tlete_drop_halt_lhs'; refinement_solver7.
-    + constructor; refinement_solver7.
-      mydestr.
-      exists x; split; auto. intros. apply IHΓ; eauto.
-      rewrite rR_shadow_update_st; refinement_solver.
-      eapply termR_perserve_rR; eauto; refinement_solver5.
-      eapply termR_tlete_drop_halt_lhs'; refinement_solver7.
-Qed.
-
-Lemma is_arr_implies_not_overbasety: forall r, is_arr r -> not_overbasety r.
-Proof.
-  intros. destruct r; invclear H; simpl; auto.
+  - constructor; refinement_solver7. mydestr. auto_meet_exists Hmeet.
+    apply IHΓ; eauto.
+    rewrite rR_shadow_update_st; refinement_solver.
+  - apply ctxrR_cons_under_arr; refinement_solver7.
+     auto_meet_exists Hmeet. invclear H7; auto_ty_exfalso.
+     rewrite ctxrR_shadow_update_st; refinement_solver.
 Qed.
 
 Global Hint Resolve is_arr_implies_not_overbasety: core.
@@ -214,25 +318,6 @@ Proof.
   eapply is_arr_simpl_rewrite_value with (P:= fun st e_x => ({st}⟦τ⟧{Γ}) (tlete e_x e)) in H1; eauto.
 Qed.
 
-Ltac auto_meet_exists HE :=
-  match goal with
-  | [H1: ({0;b∅;?st}⟦[v:?b|?n|?d|?ϕ]⟧) ?x1,
-        H2: ({0;b∅;?st}⟦[v:?b|?n|?d|?ϕ]⟧) ?x2,
-          H3: ({0;b∅;?st}⟦[v:?b|?n|?d|?ϕ]⟧) ?x3 |- ∃ e, {0;b∅;?st}⟦[v:?b|?n|?d|?ϕ]⟧ e /\ _ ] =>
-      exists ((x1 ⊗{ b } x2) ⊗{ b } x3) ; assert ( {0;b∅;st}⟦[v:b|n|d|ϕ]⟧ ((x1 ⊗{ b } x2) ⊗{ b } x3)) as HE by (eapply rR_tmeet3_when_all; auto); split; auto; intros
-  | [H1: ({0;b∅;?st}⟦[v:?b|?n|?d|?ϕ]⟧) ?x1,
-        H2: ({0;b∅;?st}⟦[v:?b|?n|?d|?ϕ]⟧) ?x2 |- ∃ e, {0;b∅;?st}⟦[v:?b|?n|?d|?ϕ]⟧ e /\ _ ] =>
-      exists (x1 ⊗{ b } x2); assert ( {0;b∅;st}⟦[v:b|n|d|ϕ]⟧ (x1 ⊗{ b } x2)) as HE by (eapply rR_tmeet_when_both; eauto); split; auto; intros
-  end.
-
-Ltac auto_meet_reduce :=
-  match goal with
-  | [H: ((?x1 ⊗{ ?b } ?x2) ⊗{ ?b } ?x3) ↪* ?v |- _ ] =>
-      rewrite reduction_tmeet3_iff_all in H; refinement_solver7; mydestr; eauto
-  | [H: (?x1 ⊗{ ?b} ?x2) ↪* ?v |- _ ] =>
-      rewrite reduction_tmeet_iff_both in H; refinement_solver7; mydestr; eauto
-  end.
-
 Ltac is_arr_simp :=
   repeat match goal with
     | [H: ∃ e_x_hat, ({0;b∅;?st}⟦?r⟧) e_x_hat /\
@@ -256,6 +341,13 @@ Ltac is_arr_simp :=
         rewrite is_arr_simpl_rewrite_ctxrR_value; auto; refinement_solver7
     end.
 
+Lemma under_not_overbasety: forall x1 x2 x3 x4, not_overbasety [v:x1|x2|x3|x4].
+Proof.
+  simpl; auto.
+Qed.
+
+Global Hint Resolve under_not_overbasety: core.
+
 Lemma rRctx_pre_weakening: forall Γ1 Γ2 st τ,
     not_overbasety τ ->
     wf_ctxrR st (Γ1 ++ Γ2) ->
@@ -263,310 +355,568 @@ Lemma rRctx_pre_weakening: forall Γ1 Γ2 st τ,
 Proof.
   induction Γ1; intros; RD_simp; denotation_simp.
   - apply rRctx_pre_weakening_empty; auto.
-  - invclear H1; invclear H0; try auto_ty_exfalso2.
+  - invclear H1; invclear H0; auto_ty_exfalso.
     + constructor; refinement_solver. basic_typing_solver7. ctx_erase_simp5.
-    + denotation_simp. invclear H9; try auto_ty_exfalso4.
+    + denotation_simp. invclear H9; try auto_ty_exfalso.
       constructor; auto. refinement_solver. ctx_erase_simp5. basic_typing_solver7. ctx_erase_simp5.
-      auto_meet_exists Hmeet2. auto_meet_reduce.
-    + invclear H9; try auto_ty_exfalso4. apply ctxrR_cons_under_arr; auto.
-      denotation_simp. refinement_solver.
-      ctx_erase_simp. basic_typing_solver7. refinement_solver7.
+      auto_meet_exists Hmeet. auto_meet_reduce.
+    + invclear H9; auto_ty_exfalso4. apply ctxrR_cons_under_arr; auto.
+      refinement_solver.
+      ctx_erase_simp. basic_typing_solver7. listctx_set_simpl. rewrite ok_pre_destruct. split; refinement_solver7.
       is_arr_simp.
 Qed.
 
-(* Ltac auto_under_specialize He := *)
-(*   repeat match goal with *)
-(*     | [H: forall e_x, _ e_x -> _ |- _ ] => specialize (H _ He) *)
-(*     | [H: forall c_x, _ (tvalue (vconst c_x)) -> _ |- _ ] => specialize (H _ He) *)
-(*     end. *)
+Lemma rR_implies_reduction_no_free_unfold
+     : ∀ (st : state) (r : rty) (e : tm) (v : value), ({0;b∅;st}⟦r⟧) e → e ↪* v → fv_value v ≡ ∅.
+Proof.
+  intros. eapply rR_implies_reduction_no_free in H; eauto.
+Qed.
 
-Ltac auto_under_specialize e :=
-  repeat match goal with
-    | [He: ?P e, H: forall e_x, ?P e_x -> _ |- _ ] => specialize (H _ He)
-    | [He: ?P (tvalue e), H: forall e_x, _ (tvalue e_x) -> _ |- _ ] => specialize (H _ He)
-    | [He: ?P (tvalue (vconst e)), H: forall c_x, _ (tvalue (vconst c_x)) -> _ |- _ ] => specialize (H _ He)
+Global Hint Resolve rR_implies_reduction_no_free_unfold: core.
+
+Lemma rR_implies_no_free_value_unfold
+     : ∀ (st : state) (r : rty) (v : value), ({0;b∅;st}⟦r⟧) v → fv_value v ≡ ∅.
+Proof.
+  intros.
+  assert ([] ⊢t v ⋮v ⌊ r ⌋); refinement_solver. basic_typing_solver.
+Qed.
+
+Global Hint Resolve rR_implies_no_free_value_unfold: core.
+
+Lemma rR_implies_no_free_value
+     : ∀ (st : state) (r : rty) (v : value), ({0;b∅;st}⟦r⟧) v → closed_value v.
+Proof.
+  intros. unfold closed_value. eapply rR_implies_no_free_value_unfold; eauto.
+Qed.
+
+Global Hint Resolve rR_implies_no_free_value: core.
+
+Ltac refinement_solver8 :=
+  match goal with
+  | [H: ok_dctx _ ((?a, ?b) :: ?c ++ _) |- ok_dctx _ ((?a, ?b) :: ?c) ] =>
+      rewrite app_comm_cons in H;
+      rewrite ok_dctx_post_destruct in H; mydestr; auto
+  | [H: {0;b∅;?st}⟦?r⟧ (tvalue ?v_x) |- _ ∉ fv_value ?v_x ] =>
+      assert ([] ⊢t v_x ⋮t ⌊ r ⌋ ) by refinement_solver7; basic_typing_solver
+  end || refinement_solver7.
+
+Ltac dsimp1 :=
+  match goal with
+  | [H: ({0;b∅;_}⟦[v:?b|_|_|_]⟧) ?e, H': ?e ↪* (tvalue ?v) |- _ ] =>
+      assert ([] ⊢t v ⋮v b) by refinement_solver; denotation_simp3
+  end.
+
+Fixpoint ty_inhabitant (t: ty): value :=
+  match t with
+  | TBase TNat => (vconst 1)
+  | TBase TBool => (vconst true)
+  | T1 ⤍ T2 => vlam T1 (ty_inhabitant T2)
+  end.
+
+Lemma closed_ty_inhabitant: forall T, fv_value (ty_inhabitant T) ≡ ∅.
+Proof.
+  induction T; simpl; intros; auto.
+  - destruct b; constructor; auto.
+Qed.
+
+Global Hint Resolve closed_ty_inhabitant: core.
+
+Lemma lc_ty_inhabitant: forall T, lc (ty_inhabitant T).
+Proof.
+  induction T; simpl; intros; auto.
+  - destruct b; constructor; auto.
+  - apply lc_vlam with (L := ∅). intros.
+    rewrite open_rec_lc_tm; auto.
+Qed.
+
+Global Hint Resolve lc_ty_inhabitant: core.
+
+Lemma ty_inhabitant_typable: forall Γ T, ok Γ -> Γ ⊢t (ty_inhabitant T) ⋮v T.
+Proof.
+  induction T; simpl; intros; auto.
+  - destruct b; constructor; auto.
+  - auto_exists_L; intros. rewrite open_rec_lc_tm; auto.
+    apply basic_typing_weaken_tm_pre; auto.
+Qed.
+
+Global Hint Resolve ty_inhabitant_typable: core.
+
+Lemma cons_basic_strengthen_tm: forall x Tx Γ1 Γ2 e T,
+    x ∉ fv_tm e ->
+    (Γ1 ++ (x, Tx) :: Γ2) ⊢t e ⋮t T ->
+    (Γ1 ++ Γ2) ⊢t e ⋮t T.
+Proof.
+  intros. apply basic_typing_subst_tm with (u:= ty_inhabitant Tx) in H0; auto.
+  - rewrite subst_fresh_tm in H0; auto.
+  - apply ty_inhabitant_typable. basic_typing_solver.
+Qed.
+
+Lemma cons_basic_strengthen_value: forall x Tx Γ1 Γ2 e T,
+    x ∉ fv_value e ->
+    (Γ1 ++ (x, Tx) :: Γ2) ⊢t e ⋮v T ->
+    (Γ1 ++ Γ2) ⊢t e ⋮v T.
+Proof.
+  intros. apply basic_typing_subst_value with (u:= ty_inhabitant Tx) in H0; auto.
+  - rewrite subst_fresh_value in H0; auto.
+  - apply ty_inhabitant_typable. basic_typing_solver.
+Qed.
+
+Lemma cons_basic_strengthen2_tm: forall Γ2 Γ1 e T,
+    ctxdom Γ2 ∩ fv_tm e ≡ ∅ ->
+    (Γ1 ++ Γ2) ⊢t e ⋮t T ->
+    Γ1 ⊢t e ⋮t T.
+Proof.
+  induction Γ2; simpl; intros; auto; mydestr.
+  - listctx_set_simpl.
+  - apply cons_basic_strengthen_tm in H0; auto. apply IHΓ2; auto. set_solver. set_solver.
+Qed.
+
+Lemma cons_basic_strengthen2_value: forall Γ2 Γ1 e T,
+    ctxdom Γ2 ∩ fv_value e ≡ ∅ ->
+    (Γ1 ++ Γ2) ⊢t e ⋮v T ->
+    Γ1 ⊢t e ⋮v T.
+Proof.
+  induction Γ2; simpl; intros; auto; mydestr.
+  - listctx_set_simpl.
+  - apply cons_basic_strengthen_value in H0; auto. apply IHΓ2; auto. set_solver. set_solver.
+Qed.
+
+Lemma cons_basic_strengthen_pre_cons_tm: forall x Tx Γ1 Γ2 e T,
+    ctxdom Γ2 ∩ fv_tm e ≡ ∅ ->
+    ((x, Tx) :: Γ1 ++ Γ2) ⊢t e ⋮t T ->
+    ((x, Tx) :: Γ1) ⊢t e ⋮t T.
+Proof.
+  intros. rewrite app_comm_cons in H0. apply cons_basic_strengthen2_tm in H0; auto.
+Qed.
+
+Lemma cons_basic_strengthen_pre_cons_value: forall x Tx Γ1 Γ2 e T,
+    ctxdom Γ2 ∩ fv_value e ≡ ∅ ->
+    ((x, Tx) :: Γ1 ++ Γ2) ⊢t e ⋮v T ->
+    ((x, Tx) :: Γ1) ⊢t e ⋮v T.
+Proof.
+  intros. rewrite app_comm_cons in H0. apply cons_basic_strengthen2_value in H0; auto.
+Qed.
+
+Lemma cons_basic_strengthen1_pre_cons_tm: forall x Tx y Ty Γ1 e T,
+    y ∉ fv_tm e ->
+    ((x, Tx) :: Γ1 ++ [(y, Ty)]) ⊢t e ⋮t T ->
+    ((x, Tx) :: Γ1) ⊢t e ⋮t T.
+Proof.
+  intros. eapply cons_basic_strengthen_pre_cons_tm; eauto. set_solver.
+Qed.
+
+Lemma cons_basic_strengthen1_pre_cons_value: forall x Tx y Ty Γ1 e T,
+    y ∉ fv_value e ->
+    ((x, Tx) :: Γ1 ++ [(y, Ty)]) ⊢t e ⋮v T ->
+    ((x, Tx) :: Γ1) ⊢t e ⋮v T.
+Proof.
+  intros. eapply cons_basic_strengthen_pre_cons_value; eauto. set_solver.
+Qed.
+
+Lemma close_rm_fv_tm: forall x e k, x ∉ fv_tm ({k <t~ x} e).
+Proof.
+  intros x e.
+  apply (tm_mutual_rec
+           (fun (e: value) => forall k, x ∉ fv_value ({k <v~ x} e))
+           (fun (e: tm) => forall k, x ∉ fv_tm ({k <t~ x} e))
+        ); simpl; intros; auto; repeat var_dec_solver; set_solver.
+Qed.
+
+Lemma close_rm_fv_value: forall x e k, x ∉ fv_value ({k <v~ x} e).
+Proof.
+  intros x e.
+  apply (value_mutual_rec
+           (fun (e: value) => forall k, x ∉ fv_value ({k <v~ x} e))
+           (fun (e: tm) => forall k, x ∉ fv_tm ({k <t~ x} e))
+        ); simpl; intros; auto; repeat var_dec_solver; set_solver.
+Qed.
+
+Lemma close_then_subst_same_tm: forall x v_x e,
+  ({x := v_x }t (x \t\ e)) = (x \t\ e).
+Proof.
+  intros. rewrite subst_fresh_tm; auto. apply close_rm_fv_tm.
+Qed.
+
+Lemma close_then_subst_same_value: forall x v_x e,
+  ({x := v_x }v (x \v\ e)) = (x \v\ e).
+Proof.
+  intros. rewrite subst_fresh_value; auto. apply close_rm_fv_value.
+Qed.
+
+Ltac lc_simpl3 :=
+  simpl;
+  repeat (match goal with
+          | [H: ({0;b∅;_}⟦ _ ⟧) ?e_x, H': context [ {?x := _ }t ?e_x] |- _ ] =>
+              assert (x ∉ fv_tm e_x) as Htmp by (eauto; refinement_solver);
+              rewrite (subst_fresh_tm e_x x) in H'; auto; try clear Htmp
+          | [H: ({0;b∅;_}⟦ _ ⟧) ?e_x |- context [ {?x := _ }t ?e_x] ] =>
+              assert (x ∉ fv_tm e_x) as Htmp by (eauto; refinement_solver);
+              rewrite (subst_fresh_tm e_x x); auto; try clear Htmp
+          | [H: ({0;b∅;_}⟦ _ ⟧) (tvalue ?e_x), H': context [ {?x := _ }v ?e_x] |- _ ] =>
+              assert (x ∉ fv_tm e_x) as Htmp by (eauto; refinement_solver);
+              rewrite (subst_fresh_value e_x x) in H'; auto; try clear Htmp
+          | [H: ({0;b∅;_}⟦ _ ⟧) (tvalue ?e_x) |- context [ {?x := _ }v ?e_x] ] =>
+              assert (x ∉ fv_tm e_x) as Htmp by (eauto; refinement_solver);
+              rewrite (subst_fresh_value e_x x); auto; try clear Htmp
+          | [|- context [ {?x := _ }t (?x \t\ _) ] ] => rewrite close_then_subst_same_tm
+          | [H: context [ {?x := _ }t (?x \t\ _) ] |- _ ] => rewrite close_then_subst_same_tm in H
+          | [|- context [ {?x := _ }v (?x \v\ _) ] ] => rewrite close_then_subst_same_value
+          | [H: context [ {?x := _ }v (?x \v\ _) ] |- _ ] => rewrite close_then_subst_same_value in H
+          end).
+
+Lemma tlete_apply_typable_aux: forall Γ (x: atom) e_x e Tx T,
+    Γ ⊢t e_x ⋮t Tx -> (Γ ++ [(x, Tx)]) ⊢t e ⋮t T -> Γ ⊢t tlete e_x (x \t\ e) ⋮t T.
+Proof.
+  intros. auto_exists_L; intros. rewrite subst_as_close_open_tm; basic_typing_solver.
+  apply basic_has_type_renaming; auto.
+  fast_set_solver. basic_typing_solver.
+Qed.
+
+Lemma tlete_apply_typable_aux2: forall Γ (x: atom) e_x e Tx T,
+    Γ ⊢t e_x ⋮t Tx -> (Γ ++ [(x, Tx)]) ⊢t e ⋮t T -> (Γ ++ [(x, Tx)]) ⊢t tlete e_x (x \t\ e) ⋮t T.
+Proof.
+  intros. assert (ok (Γ ++ [(x, Tx)])) by basic_typing_solver.
+  eapply tlete_apply_typable_aux in H0; eauto. basic_typing_solver.
+Qed.
+
+Lemma tlete_apply_typable_aux3: forall (x: atom) e_x e Tx T,
+    [] ⊢t e_x ⋮t Tx -> [(x, Tx)] ⊢t e ⋮t T -> [(x, Tx)] ⊢t tlete e_x (x \t\ e) ⋮t T.
+Proof.
+  intros. assert (([] ++ [(x, Tx)]) ⊢t tlete e_x (x \t\ e) ⋮t T).
+  eapply tlete_apply_typable_aux2; auto. listctx_set_simpl.
+Qed.
+
+Lemma tlete_apply_typable_aux4: forall a Ta Γ (x: atom) e_x e Tx T,
+    ((a, Ta):: Γ) ⊢t e_x ⋮t Tx -> ((a, Ta) :: Γ ++ [(x, Tx)]) ⊢t e ⋮t T ->
+    ((a, Ta):: Γ ++ [(x, Tx)]) ⊢t tlete e_x (x \t\ e) ⋮t T.
+Proof.
+  intros. rewrite app_comm_cons in H0. rewrite app_comm_cons.
+  eapply tlete_apply_typable_aux2; auto.
+Qed.
+
+Ltac ctx_rm_simp1 :=
+  repeat
+    match goal with
+    | [H: context [⦑(_, _) :: _⦒] |- _ ] => simpl in H; try dec_solver2
+    | [|- context [⦑(_, _) :: _⦒] ] => simpl; try dec_solver2
+    | [H: context [⦑ ?a ++ ?b ⦒] |- _ ] => setoid_rewrite (ctx_rm_app a b) in H
+    | [|- context [⦑ ?a ++ ?b ⦒] ] => setoid_rewrite (ctx_rm_app a b)
+    | [H: context [ctxdom ((_, _) :: _)] |- _] => simpl in H
+    | [|- context [ctxdom ((_, _) :: _)]] => simpl
+    | [H: context [ctxdom (_ ++ _)] |- _] =>  setoid_rewrite ctxdom_app_union in H
+    | [|- context [ctxdom (_ ++ _)]] =>  setoid_rewrite ctxdom_app_union
     end.
 
-Ltac auto_under_reduction_specialize :=
-  repeat match goal with
-      | [H: forall v, ?e ↪* (tvalue _) → _, H': ?e ↪* (tvalue _) |- _ ] => specialize (H  _ H')
-      end.
-
-Ltac auto_under e :=
-  auto_under_specialize e; mydestr; auto_under_reduction_specialize.
-
-Lemma wf_implies_ctxrR_drop_last: forall Γ st x τ_x e τ,
-    wf_ctxrR st (Γ ++ [(x, τ_x)]) ->
-    closed_rty 0 (ctxdom ⦑ Γ ⦒ ∪ dom aset st) τ ->
-    x ∉ rty_fv τ -> x ∉ fv_tm e -> not_overbasety τ_x ->
-    {st}⟦τ⟧{Γ ++ [(x, τ_x)] } e ->
-    {st}⟦τ⟧{Γ} e.
+Lemma tyable_implies_fresh_tm: forall Γ e T x,
+    Γ ⊢t e ⋮t T -> x ∉ (ctxdom Γ) -> x ∉ fv_tm e.
 Proof.
-  induction Γ; intros.
-  - invclear H; invclear H4; try auto_ty_exfalso2.
-    + auto_ty_exfalso5. auto_under x0. RD_simp.
-      rewrite rR_shadow_update_st in H9; auto. admit. refinement_solver.
-    + is_arr_simp. RD_simp.
-      assert ({0;b∅;st}⟦τ_x⟧ (random_inhabitant τ_x)) as Hrandom.
-      { apply random_inhabitant_in_any_under; refinement_solver7. }
-      auto_under Hrandom.
-      admit.
-  - mydestr. invclear H; invclear H4; try auto_ty_exfalso2.
-    + constructor; auto. admit. admit. intros. auto_under c_x.
-      apply IHΓ in H18; auto. denotation_simp. refinement_solver. admit.
-    + auto_ty_exfalso5. constructor; auto. admit. admit.
-      auto_meet_exists Hmeet2. auto_meet_reduce. auto_under e_x.
-      apply IHΓ in H4; auto. admit. admit.
-Admitted.
+  intros.
+  apply basic_typing_contains_fv_tm in H. set_solver.
+Qed.
 
-(*     wf_ctxrR st (Γ ++ [(x, τ_x)]) -> *)
-(*     closed_rty 0 (ctxdom ⦑ Γ ⦒ ∪ dom aset st) τ -> *)
-(*     x ∉ rty_fv τ -> x ∉ fv_tm e -> not_overbasety τ_x -> not_overbasety τ -> *)
-(*     {st}⟦τ⟧{Γ ++ [(x, τ_x)] } e -> *)
-(*     {st}⟦τ⟧{Γ} e. *)
-
-Definition ctxrR_appliable (st: state) (Γ : listctx rty) (e_x: tm) (τ_x: rty) :=
-  (forall x τ e, wf_ctxrR st (Γ ++ [(x, τ_x)]) ->
-            {st}⟦τ_x⟧{Γ} e_x ->
-            {st}⟦τ⟧{Γ ++ [(x, τ_x)] } e -> {st}⟦τ⟧{Γ ++ [(x, τ_x)] } (tlete e_x (x \t\ e))).
-
-Lemma wf_implies_ctxrR_tlete: forall Γ st (e_x: value) b n d ϕ,
-    ctxrR_appliable st Γ e_x [v:b|n|d|ϕ].
+Lemma tyable_implies_fresh_value: forall Γ e T x,
+    Γ ⊢t e ⋮v T -> x ∉ (ctxdom Γ) -> x ∉ fv_value e.
 Proof.
-  unfold ctxrR_appliable; induction Γ; intros; mydestr; RD_simp; denotation_simp.
-  - invclear H; invclear H1; try auto_ty_exfalso; auto. invclear H1.
-    constructor; auto. admit.
-    auto_meet_exists Hmeet3. auto_meet_reduce. auto_under e_x0. RD_simp. simpl. admit.
-  - invclear H; invclear H0; invclear H1; try auto_ty_exfalso2; auto.
-    + constructor; auto. admit. intros. auto_under c_x.
-      eapply IHΓ in H18; eauto. fold value_subst in H18. simpl. admit.
-    + auto_ty_exfalso5. constructor; auto. admit.
-      auto_meet_exists Hmeet3. auto_meet_reduce. auto_under e_x0.
-      eapply IHΓ in H0; eauto.
-Admitted.
+  intros.
+  apply basic_typing_contains_fv_value in H. set_solver.
+Qed.
 
-Lemma wf_implies_ctxrR_tlete_arr: forall Γ st (e_x: value) τ,
-    is_arr τ -> ctxrR_appliable st Γ e_x τ.
+Lemma rty_open_perserve_erase: forall τ x k, ⌊{k ~r> x} τ ⌋ = ⌊τ⌋.
 Proof.
-  unfold ctxrR_appliable; induction Γ; intros; mydestr; RD_simp; denotation_simp.
-  - invclear H0; invclear H2; try auto_ty_exfalso; auto.
-    apply ctxrR_cons_under_arr; auto. admit.
-    is_arr_simp. intros. auto_under e_x0. RD_simp. admit.
-  - invclear H0; invclear H1; invclear H2; try auto_ty_exfalso2; auto.
-    + constructor; auto. admit. intros. auto_under c_x.
-      eapply IHΓ in H19; eauto. fold value_subst in H19.
-      admit.
-    + auto_ty_exfalso5. constructor; auto. admit.
-      auto_meet_exists Hmeet3. auto_meet_reduce. auto_under e_x0.
-      apply IHΓ with (e_x:=vlam x1 (mk_app (tlete e_x0 (a \t\ e_x)) 0)) in H1; eauto. admit. admit. admit.
-    + auto_ty_exfalso.
-    + auto_ty_exfalso.
-    + apply ctxrR_cons_under_arr; auto. admit.
-      is_arr_simp. intros. auto_under e_x0.
-      apply IHΓ with (e_x:=e_x) in H21; eauto.
-      admit. admit. admit.
-Admitted.
+  induction τ; simpl; intros; auto.
+  - rewrite IHτ; auto.
+  - rewrite IHτ1; auto. rewrite IHτ2; auto.
+Qed.
 
-Definition ctxrR_appliable (st: state) (Γ : listctx rty) (e_x: tm) (τ_x: rty) :=
-  (forall x τ e, wf_ctxrR st (Γ ++ [(x, τ_x)]) ->
-            {st}⟦τ_x⟧{Γ} e_x ->
-            {st}⟦τ⟧{Γ ++ [(x, τ_x)] } e -> {st}⟦τ⟧{Γ ++ [(x, τ_x)] } (tlete e_x (x \t\ e))).
-
-Lemma wf_implies_ctxrR_tlete: forall Γ st (e_x: value) τ,
-    is_arr τ -> wf_ctxrR st Γ -> ctxrR_appliable st Γ e_x τ.
+Lemma open_subst_same_rset: forall x (v: constant) d, x ∉ d -> refinement_set_subst x v ({[x]} ∪ d) = d.
 Proof.
-  unfold ctxrR_appliable; induction Γ; intros; mydestr; RD_simp; denotation_simp.
-  - invclear H1; invclear H3; try auto_ty_exfalso; auto.
-    apply ctxrR_cons_under_arr; auto. admit.
-    is_arr_simp. intros. auto_under e_x0. RD_simp. admit.
-  - invclear H1; invclear H2; invclear H3; try auto_ty_exfalso2; auto.
-    + constructor; auto. admit. intros. auto_under c_x.
-      eapply IHΓ in H20; eauto. fold value_subst in H20.
-      admit. admit.
-    + auto_ty_exfalso5. constructor; auto. admit.
-      auto_meet_exists Hmeet3. auto_meet_reduce. auto_under e_x0.
-      apply IHΓ with (e_x:=e_x) in H2; eauto. admit. admit. admit.
-    + auto_ty_exfalso.
-    + auto_ty_exfalso.
-    + apply ctxrR_cons_under_arr; auto. admit.
-      is_arr_simp. intros. auto_under e_x0.
-      apply IHΓ with (e_x:=e_x) in H21; eauto.
-      admit. admit. admit.
-Admitted.
+  intros. unfold refinement_set_subst. dec_solver2. set_solver.
+Qed.
 
-(* Lemma wf_implies_ctxrR_drop_last: forall Γ st x τ_x e τ, *)
-(*     wf_ctxrR st (Γ ++ [(x, τ_x)]) -> *)
-(*     closed_rty 0 (ctxdom ⦑ Γ ⦒ ∪ dom aset st) τ -> *)
-(*     x ∉ rty_fv τ -> x ∉ fv_tm e -> not_overbasety τ_x -> not_overbasety τ -> *)
-(*     {st}⟦τ⟧{Γ ++ [(x, τ_x)] } e -> *)
-(*     {st}⟦τ⟧{Γ} e. *)
-(* Proof. *)
-(*   induction Γ; intros. *)
-(*   - invclear H; invclear H5; try auto_ty_exfalso. *)
-(*     + specialize (H12 _ H). mydestr. specialize (H5 _ H _ H6). RD_simp. *)
-(*       rewrite rR_shadow_update_st in H8; auto. admit. refinement_solver. *)
-(*     + is_arr_simp. *)
-(*       assert ({0;b∅;st}⟦τ_x⟧ (random_inhabitant τ_x)) as Hrandom. *)
-(*       { apply random_inhabitant_in_any_under; refinement_solver7. } *)
-(*       admit. *)
-(*   - mydestr. invclear H; invclear H5; try auto_ty_exfalso2. *)
-(*     + constructor; auto. admit. admit. intros. *)
-(*       specialize (H11 _ H). specialize (H19 _ H). *)
-(*       apply IHΓ in H19; auto. denotation_simp. refinement_solver. admit. *)
-(*     + auto_ty_exfalso5. constructor; auto. admit. admit. *)
-(*       auto_meet_exists Hmeet2. auto_meet_reduce. *)
-(*       specialize (H8 _ H6 _ H10). specialize (H5 _ H6 _ H13). *)
-(*       apply IHΓ  *)in H5; auto. admit. admit.
-Admitted.
-
-
-Lemma wf_implies_ctxrR_tlete: forall Γ st x τ_x e_x e τ,
-    not_overbasety τ -> not_overbasety τ_x ->
-    wf_ctxrR st (Γ ++ [(x, τ_x)]) ->
-    {st}⟦mk_eq_var ty⟧{Γ ++ [(x, τ_x)] } e_x ->
-    {st}⟦τ⟧{Γ ++ [(x, τ_x)] } e ->
-    {st}⟦τ⟧{Γ ++ [(x, τ_x)] } (tlete e_x e).
+Lemma open_subst_same_r: forall x (v: constant) d k (ϕ: refinement),
+    x ∉ d -> not_fv_in_refinement d ϕ ->
+      refinement_subst x v ({[x]} ∪ d) (refinement_open k x ϕ) = refinement_open k v ϕ.
 Proof.
-  induction Γ; intros; mydestr; RD_simp; denotation_simp.
-  - invclear H3. invclear H0.
-    + mydestr. invclear H1; try auto_ty_exfalso.
-      denotation_simp. constructor; auto. admit.
-      exists x0. split; auto. intros. eapply H3 in H6; eauto. RD_simp; auto. admit.
-    + invclear H1. auto_ty_exfalso.
-      apply ctxrR_cons_under_arr; auto. admit.
-      is_arr_simp. intros. apply H14 in H1. RD_simp; auto. admit.
-  - invclear H2; invclear H3; try auto_ty_exfalso4.
-    + invclear H1; try auto_ty_exfalso4; ctx_erase_simp.
-      constructor; auto. admit.
-      intros.
-      specialize (H13 _ H1). specialize (H19 _ H1). specialize (H14 _ H1).
-      eapply IHΓ in H19; eauto.
-    + denotation_simp. invclear H1. constructor; auto. denotation_simp. refinement_solver. admit.
-      mydestr.
-      exists ((x0 ⊗{ x6 } x1) ⊗{ x6 } x2).
-      split. apply rR_tmeet3_when_all; auto.
-      intros. rewrite reduction_tmeet3_iff_all in H13; refinement_solver7; mydestr.
-      assert (wf_ctxrR (({a↦v_x}) st) (Γ ++ [(x, τ_x)])) as Hwf by eauto.
-      assert ({({a↦v_x}) st}⟦τ_x⟧{Γ} (tlete e_x0 (a \t\ e_x))) as Hex by eauto.
-      assert (({({a↦v_x}) st}⟦τ⟧{Γ ++ [(x, τ_x)] }) (tlete e_x0 (a \t\ e))) as He by eauto.
-      assert ([] ⊢t v_x ⋮v x6). refinement_solver7. denotation_simp.
-      eapply IHΓ in He; eauto.
-      eapply termR_perserve_ctxrR; refinement_solver7.
-      eapply termR_tlete_commute_tlete; eauto; refinement_solver.
-      basic_typing_solver8.
+  intros. unfold refinement_subst. unfold refinement_open. unfold state_subst.
+  apply prop_ex3. intros.
+  dec_solver2. my_simplify_map_eq3.
+  apply H0. intros. my_simplify_map_eq3.
+Qed.
 
-      admit. denotation_simp. refinement_solver7.
-    + apply ctxrR_cons_under_arr; auto. denotation_simp. eapply let_store_typable; eauto.
-      is_arr_simp. intros.
-      specialize (H23 _ H2). specialize (H19 _ H2). specialize (H13 _ H2).
-      (* assert ([] ⊢t e_x ⋮t ⌊τ_x⌋) as Hxx by refinement_solver. *)
-      eapply IHΓ in H23; eauto. eauto.
-      assert (({st}⟦τ⟧{Γ}) (tlete e_x (x \t\ (tlete e_x0 (a \t\ e))))). {  eapply IHΓ in H23; eauto.
-      eapply IHΓ in H23; eauto.
-      eapply termR_perserve_ctxrR; refinement_solver7.
-      eapply termR_tlete_commute_tlete; eauto; refinement_solver.
-      basic_typing_solver8. admit.
-      denotation_simp.
-Admitted.
-
-
-
-Lemma wf_implies_ctxrR_tlete: forall Γ st x τ_x e_x e τ,
-    not_overbasety τ -> not_overbasety τ_x ->
-    wf_ctxrR st (Γ ++ [(x, τ_x)]) ->
-    {st}⟦τ_x⟧{Γ} e_x ->
-    {st}⟦τ⟧{Γ ++ [(x, τ_x)] } e ->
-    {st}⟦τ⟧{Γ ++ [(x, τ_x)] } (tlete e_x e).
+Lemma open_subst_same_rty: forall x (v: constant) τ k,
+    valid_rty τ ->
+    x # (rty_fv τ) -> {x := v }r ({k ~r> x} τ) = {k ~r> v} τ.
 Proof.
-  induction Γ; intros; mydestr; RD_simp; denotation_simp.
-  - invclear H3. invclear H0.
-    + mydestr. invclear H1; try auto_ty_exfalso.
-      denotation_simp. constructor; auto. admit.
-      exists x0. split; auto. intros. eapply H3 in H6; eauto. RD_simp; auto. admit.
-    + invclear H1. auto_ty_exfalso.
-      apply ctxrR_cons_under_arr; auto. admit.
-      is_arr_simp. intros. apply H14 in H1. RD_simp; auto. admit.
-  - invclear H2; invclear H3; try auto_ty_exfalso4.
-    + invclear H1; try auto_ty_exfalso4; ctx_erase_simp.
-      constructor; auto. admit.
-      intros.
-      specialize (H13 _ H1). specialize (H19 _ H1). specialize (H14 _ H1).
-      eapply IHΓ in H19; eauto.
-    + denotation_simp. invclear H1. constructor; auto. denotation_simp. refinement_solver. admit.
-      mydestr.
-      exists ((x0 ⊗{ x6 } x1) ⊗{ x6 } x2).
-      split. apply rR_tmeet3_when_all; auto.
-      intros. rewrite reduction_tmeet3_iff_all in H13; refinement_solver7; mydestr.
-      assert (wf_ctxrR (({a↦v_x}) st) (Γ ++ [(x, τ_x)])) as Hwf by eauto.
-      assert ({({a↦v_x}) st}⟦τ_x⟧{Γ} (tlete e_x0 (a \t\ e_x))) as Hex by eauto.
-      assert (({({a↦v_x}) st}⟦τ⟧{Γ ++ [(x, τ_x)] }) (tlete e_x0 (a \t\ e))) as He by eauto.
-      assert ([] ⊢t v_x ⋮v x6). refinement_solver7. denotation_simp.
-      eapply IHΓ in He; eauto.
-      eapply termR_perserve_ctxrR; refinement_solver7.
-      eapply termR_tlete_commute_tlete; eauto; refinement_solver.
-      basic_typing_solver8.
+  intros x v. induction τ; simpl; intros.
+  - rewrite open_subst_same_rset; auto. setoid_rewrite open_subst_same_r; auto.
+    invclear H. invclear H2; auto.
+  - rewrite open_subst_same_rset; auto. setoid_rewrite open_subst_same_r; auto.
+    invclear H. invclear H2; auto.
+  - rewrite open_subst_same_rset; auto; try fast_set_solver.
+    setoid_rewrite open_subst_same_r; auto; try fast_set_solver.
+    rewrite IHτ; auto; try fast_set_solver.
+    refinement_solver. invclear H. invclear H4; auto.
+  - rewrite IHτ1; auto; refinement_solver.
+    rewrite IHτ2; auto; refinement_solver.
+Qed.
 
-      admit. denotation_simp. refinement_solver7.
-    + apply ctxrR_cons_under_arr; auto. denotation_simp. eapply let_store_typable; eauto.
-      is_arr_simp. intros.
-      specialize (H23 _ H2). specialize (H19 _ H2). specialize (H13 _ H2).
-      (* assert ([] ⊢t e_x ⋮t ⌊τ_x⌋) as Hxx by refinement_solver. *)
-      eapply IHΓ in H23; eauto. eauto.
-      assert (({st}⟦τ⟧{Γ}) (tlete e_x (x \t\ (tlete e_x0 (a \t\ e))))). {  eapply IHΓ in H23; eauto.
-      eapply IHΓ in H23; eauto.
-      eapply termR_perserve_ctxrR; refinement_solver7.
-      eapply termR_tlete_commute_tlete; eauto; refinement_solver.
-      basic_typing_solver8. admit.
-      denotation_simp.
-Admitted.
-
-Lemma wf_implies_ctxrR_drop_last: forall Γ st x τ_x e_x e τ,
-    not_overbasety τ -> not_overbasety τ_x ->
-    closed_rty 0 (ctxdom ⦑Γ⦒ ∪ dom _ st) τ ->
-    wf_ctxrR st (Γ ++ [(x, τ_x)]) ->
-    x ∉ stale τ ->
-    {st}⟦τ_x⟧{Γ} e_x ->
-    {st}⟦τ⟧{Γ ++ [(x, τ_x)] } e ->
-    {st}⟦τ⟧{Γ} (tlete e_x (x \t\ e)).
+Lemma opened_term_tyable_renaming: forall Γ x Tx e T,
+    x ∉ fv_tm e ->
+    (Γ ++ [(x, Tx)]) ⊢t e ^t^ x ⋮t T ->
+    Γ ⊢t vlam Tx e ⋮v Tx ⤍ T.
 Proof.
-  induction Γ; intros; mydestr; RD_simp; denotation_simp.
-  - invclear H2; invclear H5; try auto_ty_exfalso4.
-    + denotation_simp. apply H12 in H2; mydestr. eapply H4 in H6; eauto. RD_simp.
-      rewrite rR_shadow_update_st in H10; auto.
-      refinement_solver.
-    + is_arr_simp. apply H19 in H6. RD_simp; auto.
-  - invclear H2; invclear H4; invclear H5; try auto_ty_exfalso4; ctx_erase_simp.
-    + invclear H9; auto_ty_exfalso. constructor; auto. eapply let_store_typable; eauto.
-      intros.
-      assert (wf_ctxrR (<[a:=c_x]> st) (Γ ++ [(x, τ_x)])) by auto.
-      assert (({<[a:=c_x]> st}⟦τ_x⟧{Γ}) ({a := c_x }t e_x)) by auto.
-      apply H22 in H2.
-      eapply IHΓ in H2; eauto. simpl.
-      rewrite subst_close_tm in H2; auto; refinement_solver7. refinement_solver.
-    + constructor; auto. denotation_simp. eapply let_store_typable; eauto.
-      mydestr; auto_ty_exfalso.
-      exists ((x0 ⊗{ x3 } x1) ⊗{ x3 } x2).
-      split. apply rR_tmeet3_when_all; auto.
-      intros. rewrite reduction_tmeet3_iff_all in H15; refinement_solver7; mydestr.
-      assert (wf_ctxrR (({a↦v_x}) st) (Γ ++ [(x, τ_x)])) as Hwf by eauto.
-      assert ({({a↦v_x}) st}⟦τ_x⟧{Γ} (tlete e_x0 (a \t\ e_x))) as Hex by eauto.
-      assert (({({a↦v_x}) st}⟦τ⟧{Γ ++ [(x, τ_x)] }) (tlete e_x0 (a \t\ e))) as He by eauto.
-      assert ([] ⊢t v_x ⋮v x3). refinement_solver7. denotation_simp.
-      eapply IHΓ in He; eauto.
-      eapply termR_perserve_ctxrR; refinement_solver7.
-      eapply termR_tlete_commute_tlete; eauto; refinement_solver.
-      basic_typing_solver8.
+  intros. auto_exists_L; simpl; intros.
+  apply basic_has_type_renaming with (x0:=x0) in H0.
+  rewrite open_subst_same_tm in H0; auto.
+  fast_set_solver. basic_typing_solver.
+Qed.
 
-      admit. denotation_simp. refinement_solver7.
-    + apply ctxrR_cons_under_arr; auto. denotation_simp. eapply let_store_typable; eauto.
-      is_arr_simp. intros.
-      specialize (H23 _ H2). specialize (H19 _ H2). specialize (H13 _ H2).
-      (* assert ([] ⊢t e_x ⋮t ⌊τ_x⌋) as Hxx by refinement_solver. *)
-      eapply IHΓ in H23; eauto. eauto.
-      assert (({st}⟦τ⟧{Γ}) (tlete e_x (x \t\ (tlete e_x0 (a \t\ e))))). {  eapply IHΓ in H23; eauto.
-      eapply IHΓ in H23; eauto.
-      eapply termR_perserve_ctxrR; refinement_solver7.
-      eapply termR_tlete_commute_tlete; eauto; refinement_solver.
-      basic_typing_solver8. admit.
-      denotation_simp.
-Admitted.
+Lemma rty_open_perserve_not_overbasety: forall τ k v, not_overbasety ({k ~r> v} τ) <-> not_overbasety τ.
+Proof.
+  induction τ; simpl; intros; auto.
+Qed.
+
+Lemma valid_rty_open: forall B n d ϕ (c: constant),
+    valid_rty {v:B|S n|d|ϕ} -> valid_rty {v:B|n|d|refinement_open n c ϕ}.
+Proof.
+  intros. invclear H. invclear H1. constructor; auto. constructor; auto.
+  - unfold not_fv_in_refinement in H. unfold not_fv_in_refinement. intros. apply H; auto.
+  - unfold bound_in_refinement. unfold bound_in_refinement in H0.
+    intros. unfold refinement_open. apply H0.
+    unfold bst_eq. intros. unfold bstate_insert. dec_solver1. apply H1. lia.
+Qed.
+
+Lemma bst_eq_insert_S: forall m bst bst' c, bst_eq m bst bst' -> bst_eq (S m) (<b[m:=c]> bst) (<b[m:=c]> bst').
+Proof.
+  unfold bst_eq; intros.
+  unfold bstate_insert. repeat var_dec_solver. apply H. lia.
+Qed.
+
+Lemma bst_eq_insert_same: forall m n bst bst' c, bst_eq m bst bst' -> bst_eq m (<b[n:=c]> bst) (<b[n:=c]> bst').
+Proof.
+  unfold bst_eq; intros.
+  unfold bstate_insert. repeat var_dec_solver.
+Qed.
+
+Lemma bound_in_refinement_btrans: forall n m c ϕ,
+    n ≤ S m ->
+    bound_in_refinement n ϕ ->
+    bound_in_refinement (n `min` m) (λ (bst : bstate) (st0 : state) (v : constant), ϕ (<b[m:=c]> bst) st0 v).
+Proof.
+  unfold bound_in_refinement; intros.
+  destruct (decide (n = S m)); subst.
+  - rewrite min_r in H1; try lia. apply H0. apply bst_eq_insert_S; auto.
+  - rewrite min_l in H1; try lia. apply H0. apply bst_eq_insert_same; auto.
+Qed.
+
+Lemma wf_r_btrans: forall n m c d ϕ,
+    n ≤ S m -> wf_r n d ϕ ->
+    wf_r (n `min` m) d (λ (bst : bstate) (st0 : state) (v : constant), ϕ (<b[m:=c]> bst) st0 v).
+Proof.
+  intros. invclear H0. constructor; auto.
+  - unfold not_fv_in_refinement. intros. apply H1; auto.
+  - apply bound_in_refinement_btrans; auto.
+Qed.
+
+Global Hint Resolve wf_r_btrans: core.
+
+Lemma not_overbasety_open_trans: forall τ m c,
+    not_overbasety τ -> not_overbasety ({m ~r> c} τ).
+Proof.
+  induction τ; simpl; intros; auto.
+Qed.
+
+Global Hint Resolve not_overbasety_open_trans: core.
+
+Lemma valid_rty_btrans: forall τ m (c: constant),
+  lc_rty_idx (S m) τ -> valid_rty τ -> valid_rty ({m ~r> c} τ).
+Proof.
+  induction τ; simpl; unfold refinement_open; intros.
+  - invclear H0; invclear H; constructor; eauto.
+  - invclear H0; invclear H; constructor; eauto.
+  - invclear H0; invclear H; constructor; eauto.
+  - invclear H0; invclear H; constructor; auto; fold rty_open; eauto.
+Qed.
+
+Global Hint Resolve valid_rty_btrans: core.
+
+Lemma lc_rty_idx_rty_btrans: forall τ m (c: constant),
+  lc_rty_idx (S m) τ -> lc_rty_idx m ({m ~r> c} τ).
+Proof.
+  induction τ; simpl; intros; invclear H; constructor; auto; lia.
+Qed.
+
+Global Hint Resolve lc_rty_idx_rty_btrans: core.
+
+Lemma rty_fv_open_c_eq: forall τ m (c: constant),
+    rty_fv ({m ~r> c} τ) ≡ rty_fv τ.
+Proof.
+  induction τ; simpl; unfold refinement_set_open; intros; auto.
+  - rewrite IHτ; auto.
+  - rewrite IHτ1; auto. rewrite IHτ2; auto.
+Qed.
+
+Lemma closed_rty_open_trans: forall τ m d (c: constant),
+    closed_rty (S m) d τ ->
+    closed_rty m d ({m ~r> c} τ).
+Proof.
+  induction τ; intros; invclear H; constructor; auto.
+  - rewrite rty_fv_open_c_eq; auto.
+  - rewrite rty_fv_open_c_eq; auto.
+Qed.
+
+Global Hint Resolve closed_rty_open_trans: core.
+
+Lemma closed_rty_implies_weak_bound_in_refinement_over: forall m L b n d ϕ,
+   closed_rty m L {v:b|n|d|ϕ} -> bound_in_refinement m ϕ.
+Proof.
+  intros. invclear H. invclear H0. invclear H3. invclear H1.
+  unfold bound_in_refinement in H0. unfold bound_in_refinement. intros. apply H0.
+  eapply bst_eq_trans; eauto.
+Qed.
+
+Lemma closed_rty_implies_weak_bound_in_refinement_under: forall m L b n d ϕ,
+   closed_rty m L [v:b|n|d|ϕ] -> bound_in_refinement m ϕ.
+Proof.
+  intros. invclear H. invclear H0. invclear H3. invclear H1.
+  unfold bound_in_refinement in H0. unfold bound_in_refinement. intros. apply H0.
+  eapply bst_eq_trans; eauto.
+Qed.
+
+Lemma closed_rty_destruct_oarr: forall τ m L b n d ϕ,
+  closed_rty m L (-:{v: b | n | d | ϕ}⤑ τ) <->
+    (closed_rty m L {v: b | n | d | ϕ} /\ closed_rty (S m) L τ /\ not_overbasety τ).
+Proof.
+  repeat split; intros; refinement_solver.
+  - constructor; auto.
+  - invclear H. invclear H0. constructor; auto. invclear H2; auto.
+Qed.
+
+Lemma closed_rty_destruct_arrarr: forall m L τ1 τ2,
+  closed_rty m L (τ1 ⤑ τ2) <->
+    (closed_rty m L τ1 /\ closed_rty m L τ2 /\ is_arr τ1 /\ not_overbasety τ2).
+Proof.
+  repeat split; intros; refinement_solver.
+  - invclear H; invclear H0; simpl; auto.
+  - destruct τ1; auto_ty_exfalso.
+    + constructor; auto; refinement_solver.
+    + constructor; auto; refinement_solver.
+Qed.
+
+From Coq Require Import Logic.FunctionalExtensionality.
+
+Lemma bstate_insert_push: forall m (c c_x: constant) bst, (<b[S m:=c]> (<b[↦c_x]> bst)) = (<b[↦c_x]> (<b[m:=c]> bst)).
+Proof.
+  unfold bstate_push; unfold bstate_insert; intros.
+  apply functional_extensionality. intros.
+  destruct x; repeat dec_solver2. invclear e. exfalso. apply n; auto.
+Qed.
+
+Lemma bst_eq_push: forall m (c_x: constant) bst bst',
+    bst_eq m bst bst' ->
+    bst_eq (S m) (<b[↦c_x]> bst) (<b[↦c_x]> bst').
+Proof.
+  unfold bst_eq; unfold bstate_push; intros.
+  destruct i; auto. apply H. lia.
+Qed.
+
+Ltac inv_rd_simpl0 :=
+  progress repeat
+    (ctx_erase_simp;
+     listctx_set_simpl;
+     ctx_rm_simp1;
+     my_simplify_map_eq3;
+     basic_typing_simpl1;
+     repeat match goal with
+       | [H: context [ ⌊{_ ~r> _} _ ⌋ ] |- _ ] => rewrite rty_open_perserve_erase in H
+       | [|- context [ ⌊{_ ~r> _} _ ⌋ ]] => rewrite rty_open_perserve_erase
+       | [H: closed_rty _ _ ?τ |- _ ∉ rty_fv ?τ ] => invclear H
+       end).
+
+Lemma rR_open_trans': forall τ m bst bst' st (c: constant) e,
+    bst_eq (S m) (<b[m:=c]> bst) bst' ->
+    (closed_rty (S m) (dom aset st) τ /\ ({m;bst;st}⟦{m ~r> c} τ⟧) e) <-> ({S m;bst';st}⟦τ⟧) e.
+Proof.
+  induction τ; split; intros; mydestr.
+  - invclear H1; mydestr. do 2 (split; auto).
+    eexists; split; eauto. split; auto. subst.
+    apply closed_rty_implies_weak_bound_in_refinement_over in H0.
+    eapply H0 in H. rewrite <- H; eauto.
+  - invclear H0; mydestr; subst. do 3 (split; auto).
+    + apply closed_rty_open_trans with (c:=c) in H0; auto.
+    + eexists; split; eauto. split; auto.
+      apply closed_rty_implies_weak_bound_in_refinement_over in H0.
+      eapply H0 in H. rewrite <- H in H3; eauto.
+  - invclear H1; mydestr. do 2 (split; auto).
+    intros. apply H3; auto.
+    apply closed_rty_implies_weak_bound_in_refinement_under in H0.
+    eapply H0 in H. rewrite <- H in H5; eauto.
+  - invclear H0; mydestr. do 3 (split; auto).
+    + apply closed_rty_open_trans with (c:=c) in H0; auto.
+    + intros. apply H2; auto.
+      apply closed_rty_implies_weak_bound_in_refinement_under in H0.
+      eapply H0 in H. rewrite <- H; eauto.
+  - invclear H1; mydestr. simpl in H2. simpl in H1. inv_rd_simpl0. do 2 (split; auto).
+    intros. apply IHτ with (c:=c) (bst:= (<b[↦c_x]> bst)); eauto.
+    + rewrite bstate_insert_push. apply bst_eq_push; auto.
+    + rewrite closed_rty_destruct_oarr in H0; mydestr. split; auto.
+      apply H3; auto.
+      apply closed_rty_implies_weak_bound_in_refinement_over in H0.
+      eapply H0 in H. rewrite <- H in H5; eauto.
+  - invclear H0; mydestr. inv_rd_simpl0. do 3 (split; auto).
+    apply closed_rty_open_trans with (c:=c) in H0; auto.
+    intros. rewrite closed_rty_destruct_oarr in H0; mydestr.
+    assert (ϕ bst' st c_x) as Hz.
+    { apply closed_rty_implies_weak_bound_in_refinement_over in H0.
+      eapply H0 in H. rewrite <- H; eauto. }
+    apply H2 in Hz; auto. rewrite <- IHτ in Hz; mydestr; eauto.
+    rewrite bstate_insert_push. apply bst_eq_push; auto.
+  - invclear H1; mydestr. simpl in H2. inv_rd_simpl0. do 2 (split; auto).
+    intros. rewrite closed_rty_destruct_arrarr in H0; mydestr.
+    eapply IHτ2; eauto. split; auto. apply H3. rewrite <- IHτ1 in H4; mydestr; eauto.
+  - invclear H0; mydestr. simpl in H1. inv_rd_simpl0. do 3 (split; auto).
+    apply closed_rty_open_trans with (c:=c) in H0; auto.
+    intros. rewrite closed_rty_destruct_arrarr in H0; mydestr.
+    assert (({S m;bst';st}⟦τ1⟧) v_x) as Hz by (rewrite <- IHτ1; eauto).
+    apply H2 in Hz. rewrite <- IHτ2 in Hz; mydestr; eauto.
+Qed.
+
+Lemma rR_open_trans_empty: forall τ st (c: constant) e,
+    closed_rty 1 (dom aset st) τ ->
+    ({0;b∅;st}⟦τ ^r^ c⟧) e -> {1;<b[↦c]> b∅;st}⟦τ⟧ e.
+Proof.
+  intros. rewrite <- rR_open_trans'; eauto.
+  unfold bst_eq; intros. destruct i; auto.
+Qed.
+
+Lemma ctxfind_get_last: forall a B Γ x τ_x,
+    ok ((a, B) :: ⌊Γ ++ [(x, τ_x)]⌋*) ->
+    ctxfind ((a, B) :: ⌊Γ ++ [(x, τ_x)]⌋*) x = Some ⌊τ_x⌋.
+Proof.
+  intros.
+  assert (x <> a). ctx_erase_simp.  basic_typing_solver8.
+  repeat dec_solver2. ctx_erase_simp. apply ctxfind_last_eq. ctx_erase_simp.
+Qed.
+
+Lemma var_last_typable: forall a B Γ x τ_x,
+    ok ((a, B) :: ⌊Γ ++ [(x, τ_x)]⌋*) -> ((a, B) :: ⌊Γ ++ [(x, τ_x)]⌋*) ⊢t x ⋮t ⌊τ_x⌋.
+Proof.
+  intros. constructor; auto. constructor; auto. apply ctxfind_get_last; auto.
+Qed.
+
+Lemma closed_rty_mk_eq_var: forall b x, closed_rty 0 ({[x]}) (mk_eq_var b x).
+Proof.
+  intros. constructor; eauto.
+  - do 2 (constructor; auto).
+    + unfold not_fv_in_refinement. intros. rewrite H; fast_set_solver.
+    + unfold bound_in_refinement. auto.
+  - constructor; auto.
+Qed.
+
+Lemma reduction_implies_termR: forall e e' T, e ↪* e' -> [] ⊢t e ⋮t T -> e' <-<{ []; T} e.
+Proof.
+  intros. constructor; auto.
+  - eapply multi_preservation; eauto.
+  - unfold termRraw. intros Γv. intros. invclear H1. simpl. simpl in H2.
+    eapply multistep_trans; eauto.
+Qed.
