new_proof/RDInv.v
@@ -1,0 +1,1151 @@
+From stdpp Require Import mapset.
+From stdpp Require Import natmap.
+From stdpp Require Import fin_map_dom.
+From CT Require Import CoreLangProp.
+From CT Require Import OperationalSemanticsProp.
+From CT Require Import BasicTypingProp.
+From CT Require Import SyntaxSugar.
+From CT Require Import Refinement.
+From CT Require Import RefinementTac.
+From CT Require Import RefinementDenotation.
+From CT Require Import RefinementDenotationTac.
+From CT Require Import RefinementDenotationProp.
+From CT Require Import TermOrdering.
+From Coq Require Import Logic.ClassicalFacts.
+From Coq Require Import Classical.
+
+Import Atom.
+Import CoreLang.
+Import CoreLangProp.
+Import Tactics.
+Import NamelessTactics.
+Import ListCtx.
+Import OperationalSemantics.
+Import OperationalSemanticsProp.
+Import BasicTyping.
+Import SyntaxSugar.
+Import Refinement.
+Import RefinementTac.
+Import RefinementDenotation.
+Import RefinementDenotationTac.
+Import RefinementDenotationProp.
+Import NamelessTactics.
+Import TermOrdering.
+
+Global Hint Resolve mk_eq_constant_is_not_overbasety: core.
+Global Hint Resolve mk_eq_var_is_not_overbasety: core.
+Global Hint Resolve is_arr_implies_not_overbasety: core.
+Global Hint Constructors ok_dctx: core.
+Global Hint Resolve rR_implies_no_free: core.
+Global Hint Resolve ctxrR_tlete_drop_halt_lhs: core.
+Global Hint Resolve rR_implies_reduction_no_free: core.
+Global Hint Resolve is_arr_implies_not_overbasety: core.
+Global Hint Resolve under_not_overbasety: core.
+
+Lemma wf_ctxrR_implies_ok: forall Γ, wf_ctxrR ∅ Γ -> ok Γ.
+Proof.
+  induction Γ; intros; auto.
+  invclear H; refinement_solver7.
+Qed.
+
+Global Hint Resolve wf_ctxrR_implies_ok: core.
+
+Inductive inv_ctxrR: state -> listctx rty -> rty -> tm -> Prop :=
+| inv_ctxrR_nil: forall st τ e, { st }⟦ τ ⟧ e -> inv_ctxrR st [] τ e
+| inv_ctxrR_cons_over: forall st (x: atom) B n d ϕ Γ τ (e: tm),
+    closed_rty 0 ({[x]} ∪ ctxdom ⦑Γ⦒ ∪ (dom _ st)) τ ->
+    ok_dctx (dom _ st) ((x, {v: B | n | d | ϕ}) :: Γ) ->
+    ((x, TBase B) :: (⌊Γ⌋*)) ⊢t e ⋮t ⌊τ⌋ ->
+     (forall (c_x: constant), {st}⟦ {v: B | n | d | ϕ} ⟧ c_x ->
+                         inv_ctxrR (<[ x := c_x ]> st) Γ τ ({x := c_x}t e)) ->
+     inv_ctxrR st ((x, {v: B | n | d | ϕ}) :: Γ) τ e
+| inv_ctxrR_cons_under_base: forall st (x: atom) b n d ϕ τ Γ e,
+    closed_rty 0 ({[x]} ∪ ctxdom ⦑Γ⦒ ∪ (dom _ st)) τ ->
+    ok_dctx (dom _ st) ((x, [v: b | n | d | ϕ]) :: Γ) ->
+    ((x, TBase b ) :: (⌊Γ⌋*)) ⊢t e ⋮t ⌊τ⌋ ->
+    (* (forall e_wf, {st}⟦ [v: b | n | d | ϕ] ⟧ e_wf -> (exists (v_wf: value), e_wf ↪* v_wf)) -> *)
+     (exists e_x_hat, {st}⟦ [v: b | n | d | ϕ] ⟧ e_x_hat /\
+                   (∀ (v_x: value), e_x_hat ↪* v_x ->
+                                       inv_ctxrR ({ x ↦ v_x } st) Γ τ ({x := v_x}t e))) ->
+     inv_ctxrR st ((x, [v: b | n | d | ϕ]) :: Γ) τ e
+| inv_ctxrR_cons_under_arr: forall st (x: atom) τ_x τ Γ e,
+    is_arr τ_x ->
+    closed_rty 0 (ctxdom ⦑Γ⦒ ∪ (dom _ st)) τ ->
+    ok_dctx (dom _ st) ((x, τ_x) :: Γ) ->
+    ((x, ⌊τ_x⌋ ) :: (⌊Γ⌋*)) ⊢t e ⋮t ⌊τ⌋ ->
+     (forall (v_x: value), {st}⟦ τ_x ⟧ v_x -> inv_ctxrR st Γ τ ({x := v_x}t e)) ->
+     inv_ctxrR st ((x, τ_x) :: Γ) τ e.
+
+Notation " '⅋{' st '}⟦' τ '⟧{' Γ '}' " := (inv_ctxrR st Γ τ) (at level 20, format "⅋{ st }⟦ τ ⟧{ Γ }", st constr, τ constr, Γ constr).
+
+Ltac RD_simp2 :=
+  repeat
+    (listctx_set_simpl;
+     match goal with
+     | [H: (⅋{_}⟦ _ ⟧{ [] }) _ |- _ ] => invclear H
+     | [|- (⅋{_}⟦ _ ⟧{ [] }) _ ] => constructor
+     | [H: (⅋{_}⟦_⟧{ (_, _) :: _ }) _ |- _ ] => invclear H; try auto_ty_exfalso
+     | [H: wf_ctxrR _ ((_,_) :: _ ) |- _ ] => invclear H; try auto_ty_exfalso
+     end).
+
+Ltac inv_simpl :=
+  repeat match goal with
+    | [H: ?x ∉ fv_tm ?e, H': context [({?x := _ }t ?e)] |- _ ] =>
+        setoid_rewrite (subst_fresh_tm e x) in H'; auto
+    | [H: ?x ∉ fv_tm ?e |- context [({?x := _ }t ?e)] ] =>
+        setoid_rewrite (subst_fresh_tm e x); auto
+    | [H: ?x ∉ rty_fv ?r, H': context [{0;b∅;({?x↦_}) _}⟦_⟧ _] |- _ ] =>
+        rewrite rR_shadow_update_st in H'; refinement_solver
+    | [H: ?x ∉ rty_fv ?r |- context [{0;b∅;({?x↦_}) _}⟦_⟧ _] ] =>
+        rewrite rR_shadow_update_st; refinement_solver
+    end.
+
+Definition riv (τ: rty): value :=
+  match τ with
+  | {v: _ | _ | _ | _ } => 0
+  | [v: _ | _ | _ | _ ] => 0
+  | -:{v: T1 | _ | _ | _ } ⤑ τ => vlam T1 (random_inhabitant τ)
+  | τ1 ⤑ τ2 => vlam (rty_erase τ1) (random_inhabitant τ2)
+  end.
+
+Lemma riv_in_any_under: ∀ (τ : rty) (bst : bstate) (n : nat) (st : state),
+    is_arr τ → closed_rty n (dom aset st) τ → ({n;bst;st}⟦τ⟧) (riv τ).
+Proof.
+  intros. destruct τ; auto_ty_exfalso.
+  - apply random_inhabitant_in_any_under; refinement_solver7.
+  - apply random_inhabitant_in_any_under; refinement_solver7.
+Qed.
+
+Ltac lc_solver_r :=
+  match goal with
+  | [H: ?x ∉ fv_tm ?e |- ?x ∉ fv_tm ({_ := _ }t ?e)] =>
+      rewrite fv_of_subst_tm_closed; refinement_solver
+  end.
+
+Lemma inv_implies_ctxrR_drop_last: forall Γ st x τ_x e τ,
+    wf_ctxrR st (Γ ++ [(x, τ_x)]) ->
+    closed_rty 0 (ctxdom ⦑ Γ ⦒ ∪ dom aset st) τ ->
+    x ∉ rty_fv τ -> x ∉ fv_tm e -> not_overbasety τ_x ->
+    ⅋{st}⟦τ⟧{Γ ++ [(x, τ_x)] } e ->
+    ⅋{st}⟦τ⟧{Γ} e.
+Proof.
+  induction Γ; intros.
+  - RD_simp2; mydestr.
+    + auto_under x1. RD_simp2. inv_simpl.
+    + assert ({0;b∅;st}⟦ τ_x ⟧ (riv τ_x)) by (apply riv_in_any_under; refinement_solver7).
+      auto_under (riv τ_x). RD_simp2. inv_simpl.
+  - RD_simp2.
+    + inversion H10; auto_ty_exfalso4; subst. constructor; auto. refinement_solver8.
+      denotation_simp. eapply cons_basic_strengthen1_pre_cons_tm; eauto.
+      intros. auto_under c_x.
+      apply IHΓ in H14; auto. refinement_solver. lc_solver_r.
+    + inversion H10; auto_ty_exfalso4; subst. mydestr. constructor; auto. refinement_solver8.
+      denotation_simp. eapply cons_basic_strengthen1_pre_cons_tm; eauto.
+      auto_meet_exists Hmeet. auto_meet_reduce. auto_under x0.
+      apply IHΓ in H11; auto. dsimp1. refinement_solver.
+      lc_solver_r.
+    + inversion H11; auto_ty_exfalso4; subst. denotation_simp. constructor; auto. refinement_solver8.
+      denotation_simp. eapply cons_basic_strengthen1_pre_cons_tm; eauto.
+      intros. auto_under v_x.
+      apply IHΓ in H15; auto. lc_solver_r.
+Qed.
+
+Lemma wf_implies_ctxrR_tlete_is_arr: forall Γ st x τ_x (e_x: value) e τ,
+    wf_ctxrR st (Γ ++ [(x, τ_x)]) ->
+    not_overbasety τ -> is_arr τ_x ->
+    ⅋{st}⟦τ_x⟧{Γ} e_x ->
+    ⅋{st}⟦τ⟧{Γ ++ [(x, τ_x)] } e -> ⅋{st}⟦τ⟧{Γ ++ [(x, τ_x)] } (tlete e_x (x \t\ e)).
+Proof.
+  induction Γ; intros; RD_simp2.
+  - constructor; auto. denotation_simp. eapply tlete_apply_typable_aux3; eauto; refinement_solver8.
+    intros. auto_under e_x. RD_simp2.
+    lc_simpl3. eapply termR_perserve_rR; eauto; refinement_solver.
+    apply termR_let_one_step_from_basic_type'. basic_typing_solver. fast_set_solver.
+    eapply tlete_apply_typable_aux; eauto; refinement_solver.
+  - constructor; auto. denotation_simp. eapply tlete_apply_typable_aux4; eauto; refinement_solver8.
+    intros. auto_under c_x.
+    eapply IHΓ in H13; eauto. fold value_subst in H13. lc_simpl3.
+    rewrite <- subst_close_tm; auto. refinement_solver. denotation_simp. basic_typing_solver8.
+  - constructor; auto. denotation_simp. eapply tlete_apply_typable_aux4; eauto; refinement_solver8.
+    mydestr. auto_meet_exists Hmeet. auto_meet_reduce.
+    auto_under ({a := v_x }t e_x). eapply IHΓ in H4; eauto. fold value_subst in H4. lc_simpl3.
+    rewrite <- subst_close_tm; auto. dsimp1. denotation_simp. basic_typing_solver8.
+  - constructor; auto. denotation_simp. eapply tlete_apply_typable_aux4; eauto; refinement_solver8.
+    intros. auto_under v_x.
+    eapply IHΓ in H18; eauto. fold value_subst in H18. lc_simpl3.
+    rewrite <- subst_close_tm; auto. refinement_solver8.
+    denotation_simp. basic_typing_solver8.
+Qed.
+
+Lemma inv_ctxrR_regular0:
+  forall Γ τ st e, ⅋{ st }⟦ τ ⟧{ Γ } e ->
+              closed_rty 0 (ctxdom ⦑Γ⦒ ∪ (dom _ st)) τ /\ ok_dctx (dom _ st) Γ.
+Proof.
+  induction Γ; simpl; intros; invclear H; simpl; auto; dec_solver2.
+  - apply rR_regular2 in H0; mydestr. constructor; simpl; auto.
+    + closed_rty_solver.
+Qed.
+
+Lemma inv_ctxrR_regular1:
+  forall Γ τ st e, ⅋{ st }⟦ τ ⟧{ Γ } e ->
+              (ok_dctx (dom _ st) Γ) /\
+                ctx_closed_rty (dom _ st) Γ /\
+                closed_rty 0 (ctxdom ⦑Γ⦒ ∪ (dom _ st)) τ.
+Proof.
+  intros. apply inv_ctxrR_regular0 in H. mydestr.
+  do 2 (split; auto). apply ok_dctx_regular2 in H0; mydestr; auto.
+Qed.
+
+Lemma inv_ctxrR_regular2:
+  forall Γ τ st e, ⅋{ st }⟦ τ ⟧{ Γ } e -> ⌊ Γ ⌋* ⊢t e ⋮t ⌊ τ ⌋.
+Proof.
+  induction Γ; simpl; intros; invclear H; simpl; auto.
+  - apply rR_regular2 in H0; mydestr; auto.
+Qed.
+
+Lemma inv_ctxrR_regular:
+  forall Γ τ st e, ⅋{ st }⟦ τ ⟧{ Γ } e ->
+              ⌊ Γ ⌋* ⊢t e ⋮t ⌊ τ ⌋ /\
+                (ok_dctx (dom _ st) Γ) /\
+                ctx_closed_rty (dom _ st) Γ /\
+                closed_rty 0 (ctxdom ⦑Γ⦒ ∪ (dom _ st)) τ.
+Proof.
+  intros. split.
+  - eapply inv_ctxrR_regular2; eauto.
+  - eapply inv_ctxrR_regular1; eauto.
+Qed.
+
+Lemma wf_ctxrR_regular1: ∀ (st: state) (Γ: listctx rty), wf_ctxrR st Γ → ok_dctx (dom _ st) Γ.
+Proof.
+  intros st Γ Hwf. induction Hwf; auto.
+Qed.
+
+Ltac ok_dctx_simpl1 :=
+  repeat
+    match goal with
+    | [H: wf_ctxrR _ _ |- _ ≡ _ ] => apply wf_ctxrR_regular1 in H; mydestr
+    | [H: wf_ctxrR _ _ |- _ ⊆ _ ] => apply wf_ctxrR_regular1 in H; mydestr
+    | [H: wf_ctxrR _ _ |- _ ∉ _ ] => apply wf_ctxrR_regular1 in H; mydestr
+    | [H: ok_dctx _ _ |- _ ≡ _ ] => apply ok_dctx_regular2 in H; mydestr
+    | [H: ok_dctx _ _ |- _ ⊆ _ ] => apply ok_dctx_regular2 in H; mydestr
+    | [H: ok_dctx _ _ |- _ ∉ _ ] => apply ok_dctx_regular2 in H; mydestr
+    | [H: ok ((_, _) :: _) |- _ ≡ _ ] => rewrite ok_pre_destruct in H; mydestr
+    | [H: ok ((_, _) :: _) |- _ ⊆ _ ] => rewrite ok_pre_destruct in H; mydestr
+    | [H: ok ((_, _) :: _) |- _ ∉ _ ] => rewrite ok_pre_destruct in H; mydestr
+    | [H: ok (_ ++ [(_, _)]) |- _ ≡ _ ] => rewrite ok_post_destruct in H; mydestr
+    | [H: ok (_ ++ [(_, _)]) |- _ ⊆ _ ] => rewrite ok_post_destruct in H; mydestr
+    | [H: ok (_ ++ [(_, _)]) |- _ ∉ _ ] => rewrite ok_post_destruct in H; mydestr
+    end.
+
+Ltac inv_rd_simpl1 :=
+  progress repeat
+    (ctx_erase_simp;
+     listctx_set_simpl;
+     ok_dctx_simpl1;
+     ctx_rm_simp1;
+     my_simplify_map_eq3;
+     basic_typing_simpl1;
+     repeat match goal with
+       | [H: context [ ⌊{_ ~r> _} _ ⌋ ] |- _ ] => rewrite rty_open_perserve_erase in H
+       | [|- context [ ⌊{_ ~r> _} _ ⌋ ]] => rewrite rty_open_perserve_erase
+       | [H: ⅋{_}⟦_⟧{_} _ |- _ ∉ fv_tm _] => apply inv_ctxrR_regular2 in H; mydestr
+       | [H: ⅋{_}⟦_⟧{_} _ |- _ ∉ fv_value _] => apply inv_ctxrR_regular2 in H; mydestr
+       | [H: closed_rty _ _ ?τ |- _ ∉ rty_fv ?τ ] => invclear H
+       end).
+
+Ltac inv_rd_solver1 :=
+  inv_rd_simpl1;
+  match goal with
+  | [H: ?Γ ⊢t ?e ⋮v ?T |- ?x ∉ fv_value ?e] => eapply tyable_implies_fresh_value in H; eauto
+  | [H: ?Γ ⊢t ?e ⋮t ?T |- ?x ∉ fv_tm ?e] => eapply tyable_implies_fresh_tm in H; eauto
+  end;
+  inv_rd_simpl1.
+
+(* Lemma ok_dctx_state_subst_implies_rty_subst_eq: forall Γ (a: atom) (L: aset) x b n d ϕ k (c_x: constant), *)
+(*     ok_dctx ({[a]} ∪ L) [(x, {k ~r> c_x} [v:b|n|d|ϕ])] -> *)
+(*     ok_dctx ({[a]} ∪ L) (Γ ++ [(x, ({k ~r> a} [v:b|n|d|ϕ]))]). *)
+(* Proof. *)
+(*   induction Γ; simpl; intros. *)
+(*   - invclear H; auto_ty_exfalso. constructor; auto. *)
+(*     invclear H4. constructor; auto. *)
+(*     + invclear H. constructor; auto. invclear H4. constructor; auto. *)
+(*       unfold not_fv_in_refinement; intros. unfold not_fv_in_refinement in H. *)
+(*       unfold refinement_open. unfold refinement_open in H. *)
+(*       destruct (m !! a); destruct (m' !! a). *)
+(*       apply H, *)
+
+Lemma state_subst_implies_r_susbt_eq: forall k (a: atom) ϕ bst st (c_x: constant) v,
+    refinement_open k a ϕ bst (<[a:=c_x]> st) v <-> refinement_open k c_x ϕ bst (<[a:=c_x]> st) v.
+Proof.
+  unfold refinement_open; split; intros; my_simplify_map_eq3.
+Qed.
+
+Lemma state_subst_implies_rty_subst_eq: forall (a: atom) (c_x: constant) Γ st τ x k b n d ϕ e,
+    (* closed_rty 0 (ctxdom Γ ∪ dom aset (<[a:=c_x]> st)) ({k ~r> a} [v:b|n|d|ϕ]) -> *)
+    ok_dctx (dom aset (<[a:=c_x]> st)) (Γ ++ [(x, {k ~r> a} [v:b|n|d|ϕ])]) ->
+    ok_dctx (dom aset (<[a:=c_x]> st)) (Γ ++ [(x, {k ~r> c_x} [v:b|n|d|ϕ])]) ->
+    (⅋{<[a:=c_x]> st}⟦τ⟧{Γ ++ [(x, {k ~r> c_x} [v:b|n|d|ϕ])] } e) <->
+    (⅋{<[a:=c_x]> st}⟦τ⟧{Γ ++ [(x, {k ~r> a} [v:b|n|d|ϕ])] } e).
+Proof.
+  induction Γ; split; intros; RD_simp2.
+  - mydestr. simpl. constructor; auto.
+    (* invclear H11; auto_ty_exfalso. constructor; auto. refinement_solver. *)
+    exists x0. split; auto. invclear H1; mydestr. constructor; auto. split; auto. refinement_solver.
+    intros. apply H4; auto. rewrite <- state_subst_implies_r_susbt_eq; auto.
+  - mydestr. simpl. constructor; auto.
+    (* invclear H11; auto_ty_exfalso. constructor; auto. refinement_solver. *)
+    exists x0. split; auto. invclear H1; mydestr. constructor; auto. split; auto. refinement_solver.
+    intros. apply H4; auto. rewrite state_subst_implies_r_susbt_eq; auto.
+  - constructor; auto. inv_rd_simpl1. inv_rd_simpl1. intros. auto_under c_x0.
+    assert (a0 <> a).
+    { rewrite dom_insert_simp in H. apply ok_dctx_regular in H; mydestr. set_solver. }
+    setoid_rewrite insert_commute; auto.
+    eapply IHΓ; eauto.
+    + repeat rewrite dom_insert_simp. invclear H; auto_ty_exfalso. rewrite dom_insert_simp in H15. ok_dctx_solver_slow.
+    + repeat rewrite dom_insert_simp. invclear H7; auto_ty_exfalso. rewrite dom_insert_simp in H15. ok_dctx_solver_slow.
+    + setoid_rewrite insert_commute; auto.
+  - constructor; auto. inv_rd_simpl1. inv_rd_simpl1. intros. auto_under c_x0. mydestr.
+    assert (a0 <> a).
+    { rewrite dom_insert_simp in H. apply ok_dctx_regular in H; mydestr. set_solver. }
+    exists x0. split; auto. intros. auto_under v_x. dsimp1.
+    setoid_rewrite insert_commute; auto.
+    eapply IHΓ; eauto.
+    + repeat rewrite dom_insert_simp. invclear H; auto_ty_exfalso. ok_dctx_solver_slow.
+    + repeat rewrite dom_insert_simp. invclear H7; auto_ty_exfalso. ok_dctx_solver_slow.
+    + setoid_rewrite insert_commute; auto.
+  - constructor; auto. inv_rd_simpl1. inv_rd_simpl1. intros. auto_under v_x.
+    eapply IHΓ; eauto.
+    + repeat rewrite dom_insert_simp. invclear H; auto_ty_exfalso. ok_dctx_solver_slow.
+    + repeat rewrite dom_insert_simp. invclear H0; auto_ty_exfalso. ok_dctx_solver_slow.
+  - constructor; auto. inv_rd_simpl1. inv_rd_simpl1. intros. auto_under c_x0.
+    assert (a0 <> a).
+    { rewrite dom_insert_simp in H. apply ok_dctx_regular in H; mydestr. set_solver. }
+    setoid_rewrite insert_commute; auto.
+    eapply IHΓ; eauto.
+    + repeat rewrite dom_insert_simp. invclear H; auto_ty_exfalso. ok_dctx_solver_slow.
+    + repeat rewrite dom_insert_simp. invclear H0; auto_ty_exfalso. ok_dctx_solver_slow.
+    + setoid_rewrite insert_commute; auto.
+  - constructor; auto. inv_rd_simpl1. inv_rd_simpl1. mydestr. exists x0. split; auto. intros.
+    auto_under v_x. dsimp1.
+    assert (a0 <> a).
+    { apply ok_dctx_regular in H; mydestr. set_solver. }
+    setoid_rewrite insert_commute; auto.
+    eapply IHΓ; eauto.
+    + repeat rewrite dom_insert_simp. invclear H; auto_ty_exfalso. ok_dctx_solver_slow.
+    + repeat rewrite dom_insert_simp. invclear H0; auto_ty_exfalso. ok_dctx_solver_slow.
+    + setoid_rewrite insert_commute; auto.
+  - constructor; auto. inv_rd_simpl1. inv_rd_simpl1. intros.
+    auto_under v_x.
+    eapply IHΓ; eauto.
+    + repeat rewrite dom_insert_simp. invclear H; auto_ty_exfalso. ok_dctx_solver_slow.
+    + repeat rewrite dom_insert_simp. invclear H0; auto_ty_exfalso. ok_dctx_solver_slow.
+Qed.
+
+Lemma state_subst_implies_rty_subst_eq': forall (a: atom) (c_x: constant) Γ st τ x k b n d ϕ e,
+    (ok_dctx (dom aset (<[a:=c_x]> st)) (Γ ++ [(x, {k ~r> a} [v:b|n|d|ϕ])]) /\
+       (⅋{<[a:=c_x]> st}⟦τ⟧{Γ ++ [(x, {k ~r> c_x} [v:b|n|d|ϕ])] } e)) <->
+    (ok_dctx (dom aset (<[a:=c_x]> st)) (Γ ++ [(x, {k ~r> c_x} [v:b|n|d|ϕ])]) /\
+       (⅋{<[a:=c_x]> st}⟦τ⟧{Γ ++ [(x, {k ~r> a} [v:b|n|d|ϕ])] } e)).
+Proof.
+  split; intros; mydestr.
+  - assert (ok_dctx (dom aset (<[a:=c_x]> st)) (Γ ++ [(x, {k ~r> c_x} [v:b|n|d|ϕ])])).
+    apply inv_ctxrR_regular in H0; mydestr; auto.
+    split; auto. rewrite <- state_subst_implies_rty_subst_eq; auto.
+  - assert (ok_dctx (dom aset (<[a:=c_x]> st)) (Γ ++ [(x, {k ~r> a} [v:b|n|d|ϕ])])).
+    apply inv_ctxrR_regular in H0; mydestr; auto.
+    split; auto. rewrite state_subst_implies_rty_subst_eq; auto.
+Qed.
+
+Lemma state_subst_implies_rty_subst_eq2: forall (a v: atom) Γ st (c_x: constant) τ x k b n d ϕ e,
+    (ok_dctx (dom aset (<[a:=c_x]> st)) (Γ ++ [(x, {k ~r> v} [v:b|n|d|ϕ])]) /\
+        ⅋{<[a:=c_x]> st}⟦τ⟧{Γ ++ [(x, {k ~r> ({a := c_x}v v)} [v:b|n|d|ϕ])] } e) <->
+    (ok_dctx (dom aset (<[a:=c_x]> st)) (Γ ++ [(x, {k ~r> ({a := c_x}v v)} [v:b|n|d|ϕ])]) /\
+       ⅋{<[a:=c_x]> st}⟦τ⟧{Γ ++ [(x, {k ~r> v} [v:b|n|d|ϕ])] } e).
+Proof.
+  intros a v. destruct (decide (a = v)).
+  - assert (forall c_x, ({a := c_x}v v) = c_x) as HJ by (simpl; intros; rewrite decide_True; auto).
+    intros. rewrite HJ. subst. rewrite state_subst_implies_rty_subst_eq'; auto.
+  - intros. rewrite subst_fresh_value; auto. fast_set_solver.
+Qed.
+
+Lemma inv_rRctx_oarr: forall Γ st (τ: rty) x b n d ϕ τ e,
+    x ∉ fv_tm e -> x ∉ rty_fv τ ->
+    wf_ctxrR st (Γ ++ [(x, {v:b|n|d|ϕ})]) ->
+    closed_rty 0 (ctxdom ⦑Γ⦒ ∪ dom _ st) (-:{v: b | n | d | ϕ}⤑ τ) ->
+    ⅋{st}⟦τ ^r^ x⟧{Γ ++ [(x, {v:b|n|d|ϕ})] } (e ^t^ x) ->
+    ⅋{st}⟦-:{v: b | n | d | ϕ}⤑ τ⟧{Γ} (vlam b e).
+Proof.
+  induction Γ; intros; RD_simp2; inv_rd_simpl1.
+  - invclear H6; auto_ty_exfalso. do 2 constructor.
+    + eapply opened_term_tyable_renaming; eauto.
+    + apply (closed_rty_trans _ (ctxdom ⦑[]⦒ ∪ dom aset st)); eauto. fast_set_solver.
+    + intros.
+      assert (({0;b∅;st}⟦{v:b|n|d|ϕ}⟧) c_x). do 2 constructor; refinement_solver.
+      auto_under c_x. RD_simp2. rewrite open_subst_same_tm in H6; auto.
+      rewrite denotation_st_update_iff_subst in H6; mydestr; try fast_set_solver.
+      rewrite open_subst_same_rty in H8; auto.
+      assert (({0;b∅;st}⟦τ0 ^r^ c_x⟧) (mk_app (vlam b e) c_x)).
+      eapply termR_perserve_rR; eauto. rewrite rty_open_perserve_not_overbasety. refinement_solver8.
+      refinement_solver.
+      apply mk_app_reduce_to_open'; refinement_solver8. inv_rd_simpl1.
+      eapply opened_term_tyable_renaming; eauto.
+      rewrite closed_rty_destruct_oarr in H2; mydestr.
+      apply rR_open_trans_empty; auto. refinement_solver.
+      refinement_solver8.
+  - invclear H9; auto_ty_exfalso. constructor; auto.
+    + refinement_solver8.
+    + simpl. constructor; auto. eapply opened_term_tyable_renaming; eauto.
+    + intros. auto_under c_x. rewrite subst_open_var_tm in H13; auto.
+      eapply IHΓ in H13; eauto.
+      pose (fv_of_subst_tm a c_x e). set_solver.
+      apply (closed_rty_trans _ ({[a]} ∪ ctxdom ⦑Γ⦒ ∪ dom aset st)); eauto. fast_set_solver.
+      refinement_solver.
+  - invclear H8; auto_ty_exfalso. constructor; auto.
+    + refinement_solver8.
+    + simpl. constructor; auto. eapply opened_term_tyable_renaming; eauto.
+    + mydestr. auto_meet_exists Hmeet. auto_meet_reduce. auto_under x0.
+      rewrite subst_open_var_tm in H8; auto.
+      eapply IHΓ in H8; eauto. dsimp1.
+      pose (fv_of_subst_tm a x3 e). set_solver.
+      apply (closed_rty_trans _ ({[a]} ∪ ctxdom ⦑Γ⦒ ∪ dom aset st)); eauto. dsimp1.
+      refinement_solver. op_solver1.
+  - invclear H10; auto_ty_exfalso. constructor; auto.
+    + refinement_solver8.
+    + simpl. constructor; auto. eapply opened_term_tyable_renaming; eauto.
+    + intros. auto_under v_x.
+      rewrite subst_open_var_tm in H14; auto.
+      eapply IHΓ in H14; eauto.
+      pose (fv_of_subst_tm a v_x e).
+      assert (fv_value v_x ≡ ∅) by refinement_solver8. set_solver.
+      refinement_solver. refinement_solver.
+Qed.
+
+Lemma inv_rRctx_arrarr: forall Γ st (τ: rty) x τ1 τ2 τ e,
+    x ∉ fv_tm e -> x ∉ rty_fv τ ->
+    wf_ctxrR st (Γ ++ [(x, τ1 ⤑ τ2)]) ->
+    closed_rty 0 (ctxdom ⦑Γ⦒ ∪ dom _ st) ((τ1 ⤑ τ2) ⤑ τ) ->
+    ⅋{st}⟦τ⟧{Γ ++ [(x, τ1 ⤑ τ2)] } (e ^t^ x) ->
+    ⅋{st}⟦(τ1 ⤑ τ2)⤑ τ⟧{Γ} (vlam ⌊τ1 ⤑ τ2⌋ e).
+Proof.
+  induction Γ; intros; RD_simp2.
+  - clear H11. invclear H10; auto_ty_exfalso. do 2 constructor.
+    + eapply opened_term_tyable_renaming; eauto.
+    + refinement_solver.
+    + intros. auto_under v_x. RD_simp2. rewrite open_subst_same_tm in H4; auto.
+      rewrite closed_rty_destruct_arrarr in H2; mydestr.
+      eapply termR_perserve_rR; eauto. refinement_solver8. simpl.
+      apply mk_app_reduce_to_open'; refinement_solver8; inv_rd_simpl1.
+      eapply opened_term_tyable_renaming; eauto.
+  - invclear H9; auto_ty_exfalso. constructor; auto.
+    + refinement_solver8.
+    + inv_rd_simpl1. constructor; auto. eapply opened_term_tyable_renaming; eauto.
+    + intros. auto_under c_x. rewrite subst_open_var_tm in H13; auto.
+      eapply IHΓ in H13; eauto.
+      pose (fv_of_subst_tm a c_x e). set_solver.
+      apply (closed_rty_trans _ ({[a]} ∪ ctxdom ⦑Γ⦒ ∪ dom aset st)); eauto. fast_set_solver.
+      refinement_solver.
+  - invclear H8; auto_ty_exfalso. constructor; auto.
+    + refinement_solver8.
+    + inv_rd_simpl1. constructor; auto. eapply opened_term_tyable_renaming; eauto.
+    + mydestr. auto_meet_exists Hmeet. auto_meet_reduce. auto_under x0.
+      rewrite subst_open_var_tm in H8; auto.
+      eapply IHΓ in H8; eauto. dsimp1.
+      pose (fv_of_subst_tm a x3 e). set_solver.
+      apply (closed_rty_trans _ ({[a]} ∪ ctxdom ⦑Γ⦒ ∪ dom aset st)); eauto. dsimp1.
+      refinement_solver. op_solver1.
+  - invclear H10; auto_ty_exfalso. constructor; auto.
+    + inv_rd_simpl1.
+    + refinement_solver8.
+    + inv_rd_simpl1. constructor; auto. eapply opened_term_tyable_renaming; eauto.
+    + inv_rd_simpl1. intros. auto_under v_x.
+      rewrite subst_open_var_tm in H14; auto.
+      eapply IHΓ in H14; eauto.
+      pose (fv_of_subst_tm a v_x e).
+      assert (fv_value v_x ≡ ∅) by refinement_solver8. set_solver.
+      refinement_solver. refinement_solver.
+Qed.
+
+Lemma inv_rRctx_pre_weakening_empty: forall Γ st τ,
+    not_overbasety τ ->
+    wf_ctxrR st Γ ->
+    (forall e, {st}⟦τ⟧ e -> ⅋{st}⟦τ⟧{Γ} e).
+Proof.
+  induction Γ; intros; RD_simp2; denotation_simp.
+  - invclear H5; auto_ty_exfalso. constructor; refinement_solver7.
+    intros. apply IHΓ; auto. lc_simpl3.
+    rewrite rR_shadow_update_st_c; refinement_solver.
+  - constructor; refinement_solver7. mydestr. auto_meet_exists Hmeet.
+    apply IHΓ; eauto.
+    rewrite rR_shadow_update_st; refinement_solver.
+    auto_under x. lc_simpl3.
+  - constructor; refinement_solver7. intros. lc_simpl3.
+Qed.
+
+Lemma inv_rRctx_pre_weakening: forall Γ1 Γ2 st τ,
+    not_overbasety τ ->
+    wf_ctxrR st (Γ1 ++ Γ2) ->
+    (forall e, ⅋{st}⟦τ⟧{Γ1} e -> ⅋{st}⟦τ⟧{Γ1 ++ Γ2} e).
+Proof.
+  induction Γ1; intros; RD_simp2; denotation_simp.
+  - apply inv_rRctx_pre_weakening_empty; auto.
+  - constructor; refinement_solver. ctx_erase_simp5. basic_typing_solver8. ctx_erase_simp5.
+  - constructor; auto. refinement_solver. ctx_erase_simp5. basic_typing_solver7. ctx_erase_simp5.
+    auto_meet_exists Hmeet. auto_meet_reduce.
+  - constructor; auto. refinement_solver. ctx_erase_simp5. basic_typing_solver7. ctx_erase_simp5.
+Qed.
+
+Lemma wf_ctxrR_implies_inv_var_is_arr_last: forall (Γ: listctx rty) st x τ_x,
+    is_arr τ_x -> closed_rty 0 (ctxdom ⦑ Γ ⦒ ∪ dom _ st) τ_x ->
+    wf_ctxrR st (Γ ++ [(x, τ_x)]) -> (⅋{st}⟦τ_x⟧{(Γ ++ [(x, τ_x)])}) x.
+Proof.
+  induction Γ; simpl; intros; mydestr.
+  - RD_simp2. constructor; auto.
+    + constructor; auto. constructor; auto. refinement_solver. simpl. var_dec_solver.
+    + intros. RD_simp2. lc_simpl3. var_dec_solver.
+  -  assert (x <> a).
+     { apply wf_ctxrR_regular1 in H1. apply ok_dctx_regular in H1; mydestr. basic_typing_solver. }
+     RD_simp2; simpl in H0.
+    + constructor; auto. inv_rd_simpl1. refinement_solver.
+      apply var_last_typable; refinement_solver.
+      intros. auto_under c_x. lc_simpl3. var_dec_solver. apply IHΓ; auto. refinement_solver8.
+    + mydestr.
+      constructor; auto. refinement_solver. apply var_last_typable; refinement_solver.
+      auto_meet_exists Hmeet. auto_under x0.
+      lc_simpl3. var_dec_solver. apply IHΓ; auto. dsimp1. refinement_solver8.
+    + constructor; auto. refinement_solver. apply var_last_typable; refinement_solver.
+      intros. lc_simpl3. var_dec_solver. apply IHΓ; auto. dec_solver2.
+Qed.
+
+Lemma wf_ctxrR_implies_inv_var_over_last: forall (Γ: listctx rty) st x b n d ϕ,
+    wf_ctxrR st (Γ ++ [(x, {v:b|n|d|ϕ})]) -> (⅋{st}⟦ mk_eq_var b x ⟧{(Γ ++ [(x, {v:b|n|d|ϕ})])}) x.
+Proof.
+  induction Γ; simpl; intros; mydestr.
+  - RD_simp2. pose (closed_rty_mk_eq_var b x). constructor; auto.
+    + refinement_solver.
+    + constructor; auto. constructor; auto. refinement_solver. simpl. var_dec_solver.
+    + intros. RD_simp2. lc_simpl3. var_dec_solver. invclear H; mydestr; subst.
+      do 2 (split; auto). denotation_simp. refinement_solver.
+      intros. my_simplify_map_eq3.
+  - pose (closed_rty_mk_eq_var b x).
+    assert (x <> a).
+    { apply wf_ctxrR_regular1 in H. apply ok_dctx_regular in H; mydestr. basic_typing_solver. }
+     RD_simp2; simpl in H0.
+    + constructor; auto. inv_rd_simpl1. refinement_solver.
+      simpl. apply var_last_typable; refinement_solver.
+      intros. auto_under c_x. lc_simpl3. var_dec_solver.
+    + mydestr.
+      constructor; auto. refinement_solver. simpl. apply var_last_typable; refinement_solver.
+      auto_meet_exists Hmeet. auto_under x0.
+      lc_simpl3. var_dec_solver.
+    + constructor; auto. refinement_solver. simpl. apply var_last_typable; refinement_solver.
+      intros. lc_simpl3. var_dec_solver.
+Qed.
+
+Lemma wf_ctxrR_implies_inv_var_under_last: forall (Γ: listctx rty) st x b n d ϕ,
+    wf_ctxrR st (Γ ++ [(x, [v:b|n|d|ϕ])]) -> (⅋{st}⟦ mk_eq_var b x ⟧{(Γ ++ [(x, [v:b|n|d|ϕ])])}) x.
+Proof.
+  induction Γ; simpl; intros; mydestr.
+  - RD_simp2. mydestr. pose (closed_rty_mk_eq_var b x). constructor; auto.
+    + refinement_solver.
+    + constructor; auto. constructor; auto. refinement_solver. simpl. var_dec_solver.
+    + auto_meet_exists Hmeet. auto_under x0. dsimp1. RD_simp2. var_dec_solver. simpl.
+      do 2 (split; auto). denotation_simp. refinement_solver.
+      intros. my_simplify_map_eq3.
+  - pose (closed_rty_mk_eq_var b x).
+    assert (x <> a).
+    { apply wf_ctxrR_regular1 in H. apply ok_dctx_regular in H; mydestr. basic_typing_solver. }
+     RD_simp2; simpl in H0.
+    + constructor; auto. inv_rd_simpl1. refinement_solver.
+      simpl. apply var_last_typable; refinement_solver.
+      intros. auto_under c_x. lc_simpl3. var_dec_solver.
+    + mydestr.
+      constructor; auto. refinement_solver. simpl. apply var_last_typable; refinement_solver.
+      auto_meet_exists Hmeet. auto_under x0.
+      lc_simpl3. var_dec_solver.
+    + constructor; auto. refinement_solver. simpl. apply var_last_typable; refinement_solver.
+      intros. lc_simpl3. var_dec_solver.
+Qed.
+
+Lemma wf_implies_ctxrR_tlete_is_arr_drop: forall Γ st x τ_x (e_x: value) e τ,
+    wf_ctxrR st (Γ ++ [(x, τ_x)]) ->
+    closed_rty 0 (ctxdom ⦑Γ⦒ ∪ dom _ st) τ ->
+    not_overbasety τ -> is_arr τ_x ->
+    ⅋{st}⟦τ_x⟧{Γ} e_x ->
+    ⅋{st}⟦τ⟧{Γ ++ [(x, τ_x)] } e -> ⅋{st}⟦τ⟧{Γ} (tlete e_x (x \t\ e)).
+Proof.
+  intros. eapply wf_implies_ctxrR_tlete_is_arr in H4; eauto.
+  eapply inv_implies_ctxrR_drop_last; eauto.
+  - inv_rd_simpl1. assert (x ∉ ctxdom ⦑Γ⦒); ctx_erase_simp. set_solver.
+  - assert (x ∉ fv_value e_x). inv_rd_solver1.
+    assert (x ∉ fv_tm (x \t\ e)) by apply close_rm_fv_tm.
+    set_solver.
+Qed.
+
+Lemma wf_implies_ctxrR_tlete_ubase: forall Γ st x b n d ϕ e_x e τ,
+    wf_ctxrR st (Γ ++ [(x, [v:b|n|d|ϕ] )]) ->
+    not_overbasety τ ->
+    ⅋{st}⟦ [v:b|n|d|ϕ] ⟧{Γ} e_x ->
+    ⅋{st}⟦τ⟧{Γ ++ [(x, [v:b|n|d|ϕ] )] } e -> ⅋{st}⟦τ⟧{Γ ++ [(x, [v:b|n|d|ϕ] )] } (tlete e_x (x \t\ e)).
+Proof.
+  induction Γ; intros; RD_simp2.
+  - constructor; auto. denotation_simp. eapply tlete_apply_typable_aux3; eauto; refinement_solver8.
+    mydestr. auto_meet_exists Hmeet. auto_meet_reduce. auto_under e_x. RD_simp2.
+    lc_simpl3. assert ([] ⊢t v_x ⋮v b) by refinement_solver.
+    assert (({0;b∅;({x↦v_x}) st}⟦τ⟧) (tlete v_x (x \t\ e))).
+    eapply termR_perserve_rR; eauto; refinement_solver.
+    apply termR_let_one_step_from_basic_type'. basic_typing_solver. fast_set_solver.
+    eapply tlete_apply_typable_aux; eauto; refinement_solver.
+    eapply termR_perserve_rR; eauto; refinement_solver.
+    eapply termR_elete; eauto.
+    eapply reduction_implies_termR; eauto. refinement_solver8.
+  - constructor; auto. denotation_simp. eapply tlete_apply_typable_aux4; eauto; refinement_solver8.
+    intros. auto_under c_x.
+    eapply IHΓ in H12; eauto. lc_simpl3.
+    rewrite <- subst_close_tm; auto. refinement_solver.
+    denotation_simp; basic_typing_solver8.
+  - constructor; auto. denotation_simp. eapply tlete_apply_typable_aux4; eauto; refinement_solver8.
+    mydestr. auto_meet_exists Hmeet. auto_meet_reduce.
+    auto_under ({a := v_x }t e_x). eapply IHΓ in H3; eauto. lc_simpl3.
+    rewrite <- subst_close_tm; auto. dsimp1.
+    denotation_simp; basic_typing_solver8.
+  - constructor; auto. denotation_simp. eapply tlete_apply_typable_aux4; eauto; refinement_solver8.
+    intros. auto_under v_x.
+    eapply IHΓ in H18; eauto. lc_simpl3.
+    rewrite <- subst_close_tm; auto. refinement_solver8.
+    denotation_simp; basic_typing_solver8.
+Qed.
+
+Lemma wf_implies_ctxrR_tlete_ubase_drop: forall Γ st x b n d ϕ e_x e τ,
+    wf_ctxrR st (Γ ++ [(x, [v:b|n|d|ϕ] )]) ->
+    closed_rty 0 (ctxdom ⦑Γ⦒ ∪ dom _ st) τ ->
+    not_overbasety τ ->
+    ⅋{st}⟦ [v:b|n|d|ϕ] ⟧{Γ} e_x ->
+    ⅋{st}⟦τ⟧{Γ ++ [(x, [v:b|n|d|ϕ] )] } e -> ⅋{st}⟦τ⟧{Γ} (tlete e_x (x \t\ e)).
+Proof.
+  intros. eapply wf_implies_ctxrR_tlete_ubase in H3; eauto.
+  eapply inv_implies_ctxrR_drop_last; eauto.
+  - inv_rd_simpl1. assert (x ∉ ctxdom ⦑Γ⦒); ctx_erase_simp. set_solver.
+  - assert (x ∉ fv_tm e_x). inv_rd_solver1.
+    assert (x ∉ fv_tm (x \t\ e)) by apply close_rm_fv_tm.
+    set_solver.
+Qed.
+
+Definition eval_op_under_bound_tm (op: biop) (a: nat) (b: nat): tm :=
+  match op with
+  | op_plus => a + b
+  | op_eq => (Nat.eqb a b)
+  | op_lt => (Nat.ltb a b)
+  | op_rannat => nat-gen
+  end.
+
+Definition eval_op_under_bound_tm_all (op: biop) (a: value) (b: value): tm :=
+  tletbiop op_eq a b (vbvar 0).
+
+Lemma eval_op_under_bound_tm_reduction_sepc: forall (op: biop) (a: nat) (b: nat) (c: constant),
+    eval_op op a b c ->
+    eval_op_under_bound_tm op a b ↪* c.
+Proof.
+  destruct op; simpl; intros; invclear H; auto.
+Qed.
+
+Global Hint Resolve eval_op_under_bound_tm_reduction_sepc: core.
+
+(* Lemma eval_op_under_bound_tm_all_reduction_sepc: forall (op: biop) (v1 v2: value) (c: constant), *)
+(*     Γ ⊢t v1 ⋮v fst_ty_of_op op -> *)
+(*     Γ ⊢t v2 ⋮v snd_ty_of_op op -> *)
+(*     eval_op op a b c -> *)
+(*     eval_op_under_bound_tm op a b ↪* c. *)
+(* Proof. *)
+(*   destruct op; simpl; intros; invclear H; auto. *)
+(* Qed. *)
+
+Lemma eval_op_under_bound_tm_reduction_sepc': forall (op: biop) (a: nat) (b: nat) (c: constant),
+    eval_op_under_bound_tm op a b ↪* c ->
+    eval_op op a b c.
+Proof.
+  destruct op; simpl; intros.
+  - rewrite value_reduce_to_value_implies_same in H; mydestr; subst.
+    invclear H. constructor.
+  - rewrite value_reduce_to_value_implies_same in H; mydestr; subst.
+    invclear H. constructor.
+  - rewrite value_reduce_to_value_implies_same in H; mydestr; subst.
+    invclear H. constructor.
+  - assert ([] ⊢t nat-gen ⋮t TNat); auto.
+    assert ([] ⊢t c ⋮t TNat). eapply multi_preservation; eauto.
+    invclear H1. invclear H4. destruct c; invclear H3. constructor.
+Qed.
+
+Global Hint Resolve eval_op_under_bound_tm_reduction_sepc': core.
+
+Lemma eval_op_under_bound_tm_tyable: forall (op: biop) (a: nat) (b: nat),
+    [] ⊢t eval_op_under_bound_tm op a b ⋮t ret_ty_of_op op.
+Proof.
+  destruct op; simpl; intros; eauto.
+  - do 2 constructor; auto.
+  - do 2 constructor; auto.
+  - do 2 constructor; auto.
+Qed.
+
+Global Hint Resolve eval_op_under_bound_tm_tyable: core.
+
+Ltac lia_dec_solver :=
+  repeat match goal with
+    | [H: context [ decide (?a = ?b) ] |- _ ] =>
+        (assert (a = b) as Htmp by lia; rewrite (decide_True _ _ Htmp) in H; try clear Htmp) ||
+          (assert (a <> b) as Htmp by lia; rewrite (decide_False _ _ Htmp) in H; try clear Htmp)
+    end.
+
+Lemma rR_eval_op_under_bound_tm: forall st (op: biop) (v1: nat) (v2: nat),
+    ({0;b∅;st}⟦[v:ret_ty_of_op op|0|∅|refinement_open 1 v2
+                                        (refinement_open 0 v1
+                                           (λ (bst : bstate) (_ : state) (v : constant),
+                                             eval_op op (bst 0) (bst 1) v))]⟧)
+      (eval_op_under_bound_tm op v1 v2).
+Proof.
+  unfold refinement_open; intros. constructor; auto; try inv_rd_simpl1.
+  do 2 (constructor; auto).
+  - do 2 (constructor; auto).
+    + unfold not_fv_in_refinement; auto.
+    + unfold bound_in_refinement. intros. unfold bstate_insert. dec_solver2.
+  - fast_set_solver.
+Qed.
+
+Lemma rR_eval_op_under_bound_tm_min: forall st (op: biop) (v1: nat) (v2: nat) e,
+    ({0;b∅;st}⟦[v:ret_ty_of_op op|0|∅|refinement_open 1 v2
+                                        (refinement_open 0 v1
+                                           (λ (bst : bstate) (_ : state) (v : constant),
+                                             eval_op op (bst 0) (bst 1) v))]⟧) e ->
+    (forall (v_x: value), eval_op_under_bound_tm op v1 v2 ↪* v_x -> e ↪* v_x).
+Proof.
+  unfold refinement_open. simpl; intros. invclear H; mydestr.
+  unfold termRraw.
+  assert ([] ⊢t eval_op_under_bound_tm op v1 v2 ⋮t ret_ty_of_op op); auto.
+  denotation_simp.
+  apply H2; refinement_solver.
+  unfold bstate_insert. dec_solver2.
+Qed.
+
+Lemma fst_ty_of_op_implies_nat:
+  forall m bst st op n d ϕ (v: value),
+    ({m;bst;st}⟦[v:fst_ty_of_op op|n|d|ϕ]⟧) v -> (exists (n: nat), v = n).
+Proof.
+  intros. invclear H; mydestr. simpl in H0. denotation_simp.
+  destruct op; destruct x; simpl in H3; invclear H3; eauto.
+Qed.
+
+Lemma tletbiop_typable: forall op (v1 v2: value) e (x: atom) T,
+    x ∉ fv_tm e ->
+    [(x, TBase (ret_ty_of_op op))] ⊢t (e ^t^ x) ⋮t T ->
+    [] ⊢t v1 ⋮v (fst_ty_of_op op) ->
+    [] ⊢t v2 ⋮v (snd_ty_of_op op) ->
+    [] ⊢t tletbiop op v1 v2 e ⋮t T.
+Proof.
+  intros.
+  econstructor; eauto. instantiate (1:= {[x]}). intros. listctx_set_simpl.
+  assert ( ([] ++ [(x, TBase (ret_ty_of_op op))]) ⊢t e ^t^ x ⋮t T) as Hz; auto.
+  apply basic_has_type_renaming with (x0:=x0) in Hz; try listctx_set_solver.
+  rewrite open_subst_same_tm in Hz; auto.
+Qed.
+
+Lemma tletbiop_typable_ctx: forall Γ op (v1 v2: value) e (x: atom) T,
+    x ∉ fv_tm e ->
+    (Γ ++ [(x, TBase (ret_ty_of_op op))]) ⊢t (e ^t^ x) ⋮t T ->
+    Γ ⊢t v1 ⋮v (fst_ty_of_op op) ->
+    Γ ⊢t v2 ⋮v (snd_ty_of_op op) ->
+    Γ ⊢t tletbiop op v1 v2 e ⋮t T.
+Proof.
+  intros. auto_exists_L; intros.
+  apply basic_has_type_renaming with (x0:=x0) in H0; try basic_typing_solver.
+  rewrite open_subst_same_tm in H0; auto.
+Qed.
+
+Lemma tletbiop_typable_ctx_dummy: forall Γ op (v1 v2: value) e (x: atom) T,
+    x ∉ fv_tm e ->
+    (Γ ++ [(x, TBase (ret_ty_of_op op))]) ⊢t (e ^t^ x) ⋮t T ->
+    Γ ⊢t v1 ⋮v (fst_ty_of_op op) ->
+    Γ ⊢t v2 ⋮v (snd_ty_of_op op) ->
+    (Γ ++ [(x, TBase (ret_ty_of_op op))]) ⊢t tletbiop op v1 v2 e ⋮t T.
+Proof.
+  intros. assert (Γ ⊢t tletbiop op v1 v2 e ⋮t T).
+  eapply tletbiop_typable_ctx; eauto. basic_typing_solver.
+Qed.
+
+Lemma tletbiop_typable_ctx_dummy_cons: forall a Ta Γ op (v1 v2: value) e (x: atom) T,
+    x ∉ fv_tm e ->
+    ((a, Ta) :: Γ ++ [(x, TBase (ret_ty_of_op op))]) ⊢t (e ^t^ x) ⋮t T ->
+    ((a, Ta) :: Γ) ⊢t v1 ⋮v (fst_ty_of_op op) ->
+    ((a, Ta) :: Γ) ⊢t v2 ⋮v (snd_ty_of_op op) ->
+    ((a, Ta) :: Γ ++ [(x, TBase (ret_ty_of_op op))]) ⊢t tletbiop op v1 v2 e ⋮t T.
+Proof.
+  intros. assert (((a, Ta) :: Γ) ⊢t tletbiop op v1 v2 e ⋮t T).
+  eapply tletbiop_typable_ctx; eauto. basic_typing_solver. listctx_set_simpl. basic_typing_solver.
+Qed.
+
+Ltac inv_rd_simpl2 :=
+  repeat match goal with
+    | [H: ⅋{_}⟦_⟧{_} _ |- _ ⊢t _ ⋮t _ ] => apply inv_ctxrR_regular2 in H; mydestr
+    | [H: ⅋{_}⟦_⟧{_} _ |- _ ⊢t _ ⋮v _] => apply inv_ctxrR_regular2 in H; mydestr
+    end.
+
+Lemma letapp_eval_op_under_bound_tm_termR: forall op (v1 v2: nat) (v_x: value) (x:atom) e T,
+    x ∉ fv_tm e ->
+    eval_op_under_bound_tm op v1 v2 ↪* v_x ->
+    [(x, TBase (ret_ty_of_op op))] ⊢t (e ^t^ x) ⋮t T ->
+    [] ⊢t (e ^t^ v_x) ⋮t T ->
+    (e ^t^ v_x) <-<{ []; T} (tletbiop op v1 v2 e).
+Proof.
+  intros. assert ([] ⊢t tletbiop op v1 v2 e ⋮t T) as Ht.
+  { econstructor; eauto. destruct op; auto. instantiate (1:= {[x]}). intros. listctx_set_simpl.
+    assert ( ([] ++ [(x, TBase (ret_ty_of_op op))]) ⊢t e ^t^ x ⋮t T) as Hz; auto.
+    apply basic_has_type_renaming with (x0:=x0) in Hz; try listctx_set_solver.
+    rewrite open_subst_same_tm in Hz; auto. }
+  constructor; auto. unfold termRraw. intros. invclear H3. simpl in H4. simpl.
+  assert ([] ⊢t (eval_op_under_bound_tm op v1 v2) ⋮t ret_ty_of_op op) as Htmp; auto.
+  assert ([] ⊢t v_x ⋮t ret_ty_of_op op). eapply multi_preservation; eauto.
+  invclear H3. invclear H7; listctx_set_simpl.
+  rewrite letbiop_step_spec. do 6 eexists; eauto.
+  assert (lc (tletbiop op v1 v2 e)) by basic_typing_solver.
+  rewrite letbiop_lc_body in H5; mydestr; auto.
+Qed.
+
+Ltac auto_meet_exists HE :=
+  match goal with
+  | [H1: ({0;b∅;?st}⟦[v:?b|?n|?d|?ϕ]⟧) ?x1,
+        H2: ({0;b∅;?st}⟦[v:?b|?n|?d|?ϕ]⟧) ?x2,
+          H3: ({0;b∅;?st}⟦[v:?b|?n|?d|?ϕ]⟧) ?x3,
+            H4: ({0;b∅;?st}⟦[v:?b|?n|?d|?ϕ]⟧) ?x4 |- ∃ e, {0;b∅;?st}⟦[v:?b|?n|?d|?ϕ]⟧ e /\ _ ] =>
+      exists (((x1 ⊗{ b } x2) ⊗{ b } x3) ⊗{ b } x4) ;
+      assert ( {0;b∅;st}⟦[v:b|n|d|ϕ]⟧ (((x1 ⊗{ b } x2) ⊗{ b } x3) ⊗{ b } x4)) as HE by (eapply rR_tmeet4_when_all; auto); split; auto; intros
+  | [H1: ({0;b∅;?st}⟦[v:?b|?n|?d|?ϕ]⟧) ?x1,
+        H2: ({0;b∅;?st}⟦[v:?b|?n|?d|?ϕ]⟧) ?x2,
+          H3: ({0;b∅;?st}⟦[v:?b|?n|?d|?ϕ]⟧) ?x3 |- ∃ e, {0;b∅;?st}⟦[v:?b|?n|?d|?ϕ]⟧ e /\ _ ] =>
+      exists ((x1 ⊗{ b } x2) ⊗{ b } x3) ; assert ( {0;b∅;st}⟦[v:b|n|d|ϕ]⟧ ((x1 ⊗{ b } x2) ⊗{ b } x3)) as HE by (eapply rR_tmeet3_when_all; auto); split; auto; intros
+  | [H1: ({0;b∅;?st}⟦[v:?b|?n|?d|?ϕ]⟧) ?x1,
+        H2: ({0;b∅;?st}⟦[v:?b|?n|?d|?ϕ]⟧) ?x2 |- ∃ e, {0;b∅;?st}⟦[v:?b|?n|?d|?ϕ]⟧ e /\ _ ] =>
+      exists (x1 ⊗{ b } x2); assert ( {0;b∅;st}⟦[v:b|n|d|ϕ]⟧ (x1 ⊗{ b } x2)) as HE by (eapply rR_tmeet_when_both; eauto); split; auto; intros
+  | [H1: ({0;b∅;?st}⟦[v:?b|?n|?d|?ϕ]⟧) ?x1 |- ∃ e, {0;b∅;?st}⟦[v:?b|?n|?d|?ϕ]⟧ e /\ _ ] =>
+      exists x1; split; eauto; intros
+  | [|- ∃ e, {0;b∅;?st}⟦?r⟧ e /\ _ ] =>
+      assert ({0;b∅;st}⟦r⟧ (random_inhabitant r)) by (apply random_inhabitant_in_any_under; refinement_solver7);
+      eexists; split; eauto; intros
+  end.
+
+Ltac auto_meet_reduce :=
+  match goal with
+  | [H: (((?x1 ⊗{ ?b } ?x2) ⊗{ ?b } ?x3) ⊗{ ?b } ?x4)↪* ?v |- _ ] =>
+      rewrite reduction_tmeet4_iff_all in H; refinement_solver7; mydestr; eauto
+  | [H: ((?x1 ⊗{ ?b } ?x2) ⊗{ ?b } ?x3) ↪* ?v |- _ ] =>
+      rewrite reduction_tmeet3_iff_all in H; refinement_solver7; mydestr; eauto
+  | [H: (?x1 ⊗{ ?b} ?x2) ↪* ?v |- _ ] =>
+      rewrite reduction_tmeet_iff_both in H; refinement_solver7; mydestr; eauto
+  end.
+
+Lemma snd_ty_of_op_implies_nat:
+  forall m bst st op n d ϕ (v: value),
+    ({m;bst;st}⟦[v:snd_ty_of_op op|n|d|ϕ]⟧) v -> (exists (n: nat), v = n).
+Proof.
+  intros. invclear H; mydestr. simpl in H0. denotation_simp.
+  destruct op; destruct x; simpl in H3; invclear H3; eauto.
+Qed.
+
+Lemma rR_basety_implies_nat:
+  forall m bst st b n d ϕ (v: value),
+    ({m;bst;st}⟦[v:b|n|d|ϕ]⟧) v -> (exists (c: constant), v = c).
+Proof.
+  intros. invclear H; mydestr. simpl in H0. denotation_simp.
+  destruct x; simpl in H; invclear H; eauto.
+Qed.
+
+Lemma has_basety_implies_constant_or_var: forall Γ (b: base_ty) (v: value),
+    Γ ⊢t v ⋮v b -> ((exists (n: constant), v = n) \/ (exists (y: atom), v = y)).
+Proof.
+  intros.
+  destruct v.
+  + left. eexists; eauto.
+  + right. eexists; eauto.
+  + invclear H.
+  + invclear H.
+  + invclear H.
+Qed.
+
+Lemma inv_basety_implies_constant_or_var: forall Γ st b n d ϕ (v: value),
+    (⅋{st}⟦[v:b|n|d|ϕ]⟧{Γ}) v -> ((exists (n: constant), v = n) \/ (exists (y: atom), v = y)).
+Proof.
+  intros. apply inv_ctxrR_regular in H; mydestr; eauto. invclear H.
+  eapply has_basety_implies_constant_or_var; eauto.
+Qed.
+
+Lemma state_subst_implies_rty_subst_eq2_forward_ok_dctx
+    : ∀ (a v : atom) (Γ : list (atom * rty)) (L : aset) (c_x : constant) (x : atom)
+      (k : nat) (b : base_ty) (n : nat) (d : aset) (ϕ : refinement),
+  not_fv_in_refinement d ϕ -> a ∈ L ->
+  bound_in_refinement (n `min` k) (refinement_open k c_x ϕ) ->
+  ok_dctx L (Γ ++ [(x, {k ~r> v} [v:b|n|d|ϕ])]) ->
+  ok_dctx L (Γ ++ [(x, {k ~r> {a := c_x }v v} [v:b|n|d|ϕ])]).
+Proof.
+  intros a v. induction Γ; intros.
+  - denotation_simp. destruct (decide (a = v)); subst; auto.
+    invclear H2; auto_ty_exfalso. constructor; auto.
+    invclear H7. constructor; auto.
+    + invclear H2. constructor; auto. invclear H7. constructor; auto.
+      unfold not_fv_in_refinement. intros. apply H. intros. apply H7; auto.
+    + invclear H3. constructor; auto.
+    + simpl in H4. simpl. set_solver.
+  - mydestr. invclear H2; auto_ty_exfalso.
+    + constructor; auto; fold (@app (atom * rty)). listctx_set_simpl.
+      eapply IHΓ; eauto. set_solver.
+    + apply ok_dctx_cons_arr; auto; fold (@app (atom * rty)). listctx_set_simpl.
+Qed.
+
+(* Lemma state_subst_implies_rty_subst_eq2_forward_ok_dctx *)
+(*     : ∀ (a v : atom) (Γ : list (atom * rty)) (L : aset) (c_x : constant) (x : atom) *)
+(*       (k : nat) (b : base_ty) (n : nat) (d : aset) (ϕ : refinement), *)
+(*   not_fv_in_refinement ∅ ϕ -> a ∈ L -> *)
+(*   bound_in_refinement (n `min` k) (refinement_open k c_x ϕ) -> *)
+(*   ok_dctx L (Γ ++ [(x, {k ~r> v} [v:b|n|d|ϕ])]) -> *)
+(*   ok_dctx L (Γ ++ [(x, {k ~r> {a := c_x }v v} [v:b|n|d|ϕ])]). *)
+(* Proof. *)
+(*   intros a v. induction Γ; intros. *)
+(*   - denotation_simp. destruct (decide (a = v)); subst; auto. *)
+(*     invclear H2; auto_ty_exfalso. constructor; auto. *)
+(*     invclear H7. constructor; auto. *)
+(*     + invclear H2. constructor; auto. invclear H7. constructor; auto. *)
+(*       unfold not_fv_in_refinement. intros. apply H. intros. invclear H8. *)
+(*     + invclear H3. constructor; auto. *)
+(*     + simpl in H4. simpl. set_solver. *)
+(*   - mydestr. invclear H2; auto_ty_exfalso. *)
+(*     + constructor; auto; fold (@app (atom * rty)). listctx_set_simpl. *)
+(*       eapply IHΓ; eauto. set_solver. *)
+(*     + apply ok_dctx_cons_arr; auto; fold (@app (atom * rty)). listctx_set_simpl. *)
+(* Qed. *)
+
+Lemma state_subst_implies_rty_subst_eq2_forward
+  : ∀ (a v : atom) (Γ : list (atom * rty)) (st : state) (c_x : constant) (τ : rty) (x : atom)
+      (k : nat) (b : base_ty) (n : nat) (d : aset) (ϕ : refinement) (e : tm),
+    ok_dctx (dom aset (<[a:=c_x]> st)) (Γ ++ [(x, {k ~r> {a := c_x }v v} [v:b|n|d|ϕ])]) ->
+    (⅋{<[a:=c_x]> st}⟦τ⟧{Γ ++ [(x, {k ~r> v} [v:b|n|d|ϕ])] }) e ->
+    (⅋{<[a:=c_x]> st}⟦τ⟧{Γ ++ [(x, {k ~r> {a := c_x }v v} [v:b|n|d|ϕ])] }) e.
+Proof.
+  intros.
+  assert (ok_dctx (dom aset (<[a:=c_x]> st)) (Γ ++ [(x, {k ~r> {a := c_x }v v} [v:b|n|d|ϕ])]) /\
+         (⅋{<[a:=c_x]> st}⟦τ⟧{Γ ++ [(x, {k ~r> v} [v:b|n|d|ϕ])] }) e). split; auto.
+  rewrite <- state_subst_implies_rty_subst_eq2 in H1; mydestr; auto.
+Qed.
+
+Lemma state_subst_implies_rty_subst_eq2_backward
+  : ∀ (a v : atom) (Γ : list (atom * rty)) (st : state) (c_x : constant) (τ : rty) (x : atom)
+      (k : nat) (b : base_ty) (n : nat) (d : aset) (ϕ : refinement) (e : tm),
+    ok_dctx (dom aset (<[a:=c_x]> st)) (Γ ++ [(x, {k ~r> v} [v:b|n|d|ϕ])]) ->
+    (⅋{<[a:=c_x]> st}⟦τ⟧{Γ ++ [(x, {k ~r> {a := c_x }v v} [v:b|n|d|ϕ])] }) e ->
+    (⅋{<[a:=c_x]> st}⟦τ⟧{Γ ++ [(x, {k ~r> v} [v:b|n|d|ϕ])] }) e.
+Proof.
+  intros.
+  assert (ok_dctx (dom aset (<[a:=c_x]> st)) (Γ ++ [(x, {k ~r> v} [v:b|n|d|ϕ])]) /\
+         (⅋{<[a:=c_x]> st}⟦τ⟧{Γ ++ [(x, {k ~r> {a := c_x }v v} [v:b|n|d|ϕ])]  }) e). split; auto.
+  rewrite state_subst_implies_rty_subst_eq2 in H1; mydestr; auto.
+Qed.
+
+Require Import Coq.Logic.FunctionalExtensionality.
+
+Lemma bstate_insert_commute: forall n1 n2 c0 c x,
+    n1 <> n2 ->
+  (<b[n2:=c0]> (<b[n1:=c]> x)) = (<b[n1:=c]> (<b[n2:=c0]> x)).
+Proof.
+  unfold bstate_insert. intros.
+  apply functional_extensionality; intros.
+  dec_solver2.
+Qed.
+
+Lemma rty_open_commute: forall n1 n2 (v1 v2: value) b d n ϕ,
+    lc v1 -> lc v2 -> n1 <> n2 ->
+    {n1 ~r> v1} ({n2 ~r> v2} [v:b|d|n|ϕ]) = {n2 ~r> v2} ({n1 ~r> v1} [v:b|d|n|ϕ]).
+Proof.
+  intros. simpl. assert ((d `min` n2) `min` n1 = (d `min` n1) `min` n2). lia. rewrite H2. clear H2.
+  assert (refinement_set_open n1 v1 (refinement_set_open n2 v2 n) = refinement_set_open n2 v2 (refinement_set_open n1 v1 n)).
+  unfold refinement_set_open.
+  destruct v1; destruct v2; auto. set_solver.
+  rewrite H2. clear H2.
+  assert (refinement_open n1 v1 (refinement_open n2 v2 ϕ) = refinement_open n2 v2 (refinement_open n1 v1 ϕ)).
+  unfold refinement_open.
+  do 3 (apply functional_extensionality; intros).
+  destruct v1; destruct v2; try destruct (x0 !! atom); try destruct (x0 !! atom0); auto;
+  rewrite bstate_insert_commute; auto.
+  rewrite H2; auto.
+Qed.
+
+Lemma tletbiop_aux1: forall op (x1:atom),
+    not_fv_in_refinement ({[x1]} ∪ ∅)
+    (refinement_open 0 x1 (λ (bst : bstate) (_ : state) (v : constant), eval_op op (bst 0) (bst 1) v)).
+Proof.
+  intros. unfold not_fv_in_refinement. intros. unfold refinement_open.
+  assert (m !! x1 = m' !! x1). apply H. set_solver.
+  rewrite H0.
+  destruct (m' !! x1); auto.
+Qed.
+
+Lemma bstate_insert_insert:
+  ∀ (n1 : nat) (c0 c : constant) (x : bstate), <b[n1:=c0]> (<b[n1:=c]> x) = <b[n1:=c0]> x.
+Proof.
+  intros. unfold bstate_insert. apply functional_extensionality; intros.
+  dec_solver2.
+Qed.
+
+Lemma mk_op_ret_ok_dctx
+    : ∀ st op (a : atom) (v1 v2: value) (Γ : list (atom * rty)) (c_x : constant) (x : atom) e τ,
+    ((exists (n: constant), v1 = n) \/ (exists (y: atom), v1 = y)) ->
+    ((exists (n: constant), v2 = n) \/ (exists (y: atom), v2 = y)) ->
+    ok_dctx (dom aset (<[a:=c_x]> st)) (Γ ++ [(x, {1 ~r> v2} (mk_op_ret op ^r^ v1))]) ->
+    (⅋{<[a:=c_x]> st}⟦τ⟧{Γ ++ [(x, {1 ~r> ({a := c_x }v v2)} (mk_op_ret op ^r^ ({a := c_x }v v1)))] } e) <->
+       (⅋{<[a:=c_x]> st}⟦τ⟧{Γ ++ [(x, {1 ~r> v2} (mk_op_ret op ^r^ v1))] }) e.
+Proof.
+  split; intros; mydestr; subst.
+  - destruct H; destruct H0; mydestr; subst; auto.
+    + destruct (decide (a = x0)); auto; subst.
+      assert ((mk_op_ret op ^r^ x1) = [v:ret_ty_of_op op|0| ∅|refinement_open 0 x1
+                                    (λ (bst : bstate) (_ : state) (v : constant), eval_op op (bst 0) (bst 1) v)]); auto.
+      rewrite H. apply state_subst_implies_rty_subst_eq2_backward; auto.
+      simpl in H2. dec_solver2.
+    + destruct (decide (a = x1)); auto; subst.
+      unfold mk_op_ret. rewrite rty_open_commute; auto.
+      unfold mk_op_ret in H1. rewrite rty_open_commute in H1; auto.
+      unfold mk_op_ret in H2. rewrite rty_open_commute in H2; auto.
+      apply state_subst_implies_rty_subst_eq2_backward; auto.
+      simpl; auto. simpl; auto. dec_solver1.
+      simpl in H2. dec_solver2.
+    + destruct (decide (a = x0)); auto; subst.
+      assert ((⅋{<[x0:=c_x]> st}⟦τ⟧{Γ ++ [(x, {1 ~r> {x0 := c_x }v x0} (mk_op_ret op ^r^ x1))] }) e).
+      { assert ({x0 := c_x }v x0 = c_x). simpl. dec_solver2.
+        rewrite H. rewrite H in H2. clear H.
+        unfold mk_op_ret in H2. rewrite rty_open_commute in H2; auto.
+        assert (ok_dctx (dom aset (<[x0:=c_x]> st)) (Γ ++ [(x, {1 ~r> c_x} (mk_op_ret op ^r^ x1))])).
+        apply state_subst_implies_rty_subst_eq2_forward_ok_dctx with (a:=x0) (c_x :=c_x) in H1; eauto.
+        simpl in H1. rewrite decide_True in H1; auto. unfold refinement_set_open. apply tletbiop_aux1; auto.
+        rewrite dom_insert_simp. set_solver. admit.
+        (* - assert ((2 `min` 0) `min` 1 = 0) by lia. rewrite H. clear H. *)
+        (*   rewrite ok_dctx_post_destruct in H1; mydestr. invclear H3. invclear H4. invclear H7. *)
+        (*   unfold bound_in_refinement. intros. unfold bound_in_refinement in H4. *)
+        (*   specialize (H4 _ _ st0 v H7). admit. *)
+        (* -  *)
+        unfold mk_op_ret in H. rewrite rty_open_commute in H; auto.
+        unfold mk_op_ret. rewrite rty_open_commute; auto.
+        destruct (decide (x0 = x1)); auto; subst.
+        apply state_subst_implies_rty_subst_eq2_backward; auto.
+        simpl in H2. dec_solver2.
+        simpl. dec_solver2.
+      }
+      apply state_subst_implies_rty_subst_eq2_backward; auto.
+      assert ({a := c_x }v x0 = x0). simpl. dec_solver1; auto.
+      rewrite H in H2. clear H.
+      unfold mk_op_ret in H2. rewrite rty_open_commute in H2; auto.
+      unfold mk_op_ret in H1. rewrite rty_open_commute in H1; auto.
+      unfold mk_op_ret. rewrite rty_open_commute; auto.
+      apply state_subst_implies_rty_subst_eq2_backward; auto.
+      simpl; auto. dec_solver1.
+Admitted.
+
+Lemma inv_rRctx_tletbiop: forall Γ st (τ: rty) x op n1 d1 ϕ1 n2 d2 ϕ2 (v1 v2: value) e,
+    x ∉ fv_tm e -> x ∉ rty_fv τ -> not_overbasety τ ->
+    wf_ctxrR st (Γ ++ [(x, {1 ~r> v2} (mk_op_ret op ^r^ v1))]) ->
+    (⅋{st}⟦[v:fst_ty_of_op op|n1|d1|ϕ1]⟧{Γ}) v1 ->
+    (⅋{st}⟦[v:snd_ty_of_op op|n2|d2|ϕ2]⟧{Γ}) v2 ->
+    (⅋{st}⟦τ⟧{Γ ++ [(x, {1 ~r> v2} (mk_op_ret op ^r^ v1))] }) (e ^t^ x) ->
+    ⅋{st}⟦τ⟧{Γ ++ [(x, {1 ~r> v2} (mk_op_ret op ^r^ v1))] } (tletbiop op v1 v2 e).
+Proof.
+  induction Γ; intros; RD_simp2.
+  - mydestr. inv_rd_simpl1. constructor; auto.
+    + denotation_simp. assert ([] ⊢t tletbiop op v1 v2 e ⋮t ⌊τ⌋). eapply tletbiop_typable; refinement_solver.
+      basic_typing_solver.
+    + assert ((exists (m1: nat), v1 = m1)) by (eapply fst_ty_of_op_implies_nat; eauto). mydestr; subst. rename x2 into v1.
+      assert ((exists (m2: nat), v2 = m2)) by (eapply snd_ty_of_op_implies_nat; eauto). mydestr; subst. rename x2 into v2.
+      exists (eval_op_under_bound_tm op v1 v2). split. apply rR_eval_op_under_bound_tm.
+      intros. assert (x1 ↪* v_x) as Hz by (eapply rR_eval_op_under_bound_tm_min; eauto).
+      auto_under v_x. RD_simp2. simpl.
+      rewrite subst_fresh_tm; auto. rewrite open_subst_same_tm in H10; auto.
+      eapply termR_perserve_rR; refinement_solver.
+      eapply letapp_eval_op_under_bound_tm_termR; eauto; refinement_solver.
+  - constructor; auto. denotation_simp. apply tletbiop_typable_ctx_dummy_cons; auto.
+    intros. auto_under c_x. invclear H11; auto_ty_exfalso.
+    assert ((exists (n: constant), v1 = n) \/ (exists (y: atom), v1 = y)).
+    { invclear H20. eapply has_basety_implies_constant_or_var; eauto. }
+    assert ((exists (n: constant), v2 = n) \/ (exists (y: atom), v2 = y)).
+    { invclear H23. eapply has_basety_implies_constant_or_var; eauto. }
+    assert ((⅋{<[a:=c_x]> st}⟦τ⟧{Γ ++ [(x, {1 ~r> ({a := c_x }v v2)} (mk_op_ret op ^r^ ({a := c_x }v v1)))] }) ({a := c_x }t tletbiop op v1 v2 e)).
+    { eapply IHΓ; eauto; fold value_subst.
+      rewrite fv_of_subst_tm_closed; refinement_solver. admit.
+      fold tm_subst. rewrite <- subst_open_var_tm; auto. admit.
+      denotation_simp. }
+    admit.
+  - constructor; auto. denotation_simp. apply tletbiop_typable_ctx_dummy_cons; auto.
+    mydestr. auto_meet_exists Hmeet. auto_meet_reduce. auto_under v_x. simpl.
+    eapply IHΓ; eauto; fold tm_subst.
+    + rewrite fv_of_subst_tm_closed; refinement_solver.
+    + rewrite <- subst_open_var_tm; auto. denotation_simp. basic_typing_solver. op_solver1.
+  - constructor; auto. denotation_simp. apply tletbiop_typable_ctx_dummy_cons; auto.
+    intros. auto_under v_x. eapply IHΓ; eauto; fold tm_subst.
+    + rewrite fv_of_subst_tm_closed; refinement_solver.
+    + rewrite <- subst_open_var_tm; auto. denotation_simp. basic_typing_solver. refinement_solver.
+
+
+
+    destruct H3; destruct H4; mydestr; subst.
+    + eapply IHΓ; eauto.
+      rewrite fv_of_subst_tm_closed; refinement_solver.
+      rewrite <- subst_open_var_tm; auto. denotation_simp. basic_typing_solver.
+    + simpl. destruct (decide (a = x0)).
+      eapply IHΓ; eauto.
+
+      eapply state_subst_implies_rty_subst_eq2_forward; auto. admit.
+      apply inv_ctxrR_regular in H15; mydestr; auto.
+      eapply IHΓ; eauto.
+      rewrite fv_of_subst_tm_closed; refinement_solver.
+      rewrite <- subst_open_var_tm; auto. denotation_simp. basic_typing_solver.
+
+    eapply has_basety_implies_constant_or_var; eauto. apply H20.
+    Check state_subst_implies_rty_subst_eq2.
+    rewrite state_subst_implies_rty_subst_eq2.
+
+    eapply IHΓ; eauto.
+    + rewrite fv_of_subst_tm_closed; refinement_solver.
+    + rewrite <- subst_open_var_tm; auto. denotation_simp. basic_typing_solver.
+  - constructor; auto. denotation_simp. apply tletbiop_typable_ctx_dummy_cons; auto.
+    mydestr. auto_meet_exists Hmeet. auto_meet_reduce. auto_under v_x. eapply IHΓ; eauto; fold tm_subst.
+    + rewrite fv_of_subst_tm_closed; refinement_solver.
+    + rewrite <- subst_open_var_tm; auto. denotation_simp. basic_typing_solver. op_solver1.
+  - constructor; auto. denotation_simp. apply tletbiop_typable_ctx_dummy_cons; auto.
+    intros. auto_under v_x. eapply IHΓ; eauto; fold tm_subst.
+    + rewrite fv_of_subst_tm_closed; refinement_solver.
+    + rewrite <- subst_open_var_tm; auto. denotation_simp. basic_typing_solver. refinement_solver.
+Qed.
+
+
+Lemma inv_rRctx_tletbiop: forall Γ st (τ: rty) x op n1 d1 ϕ1 n2 d2 ϕ2 (v1 v2: nat) e,
+    x ∉ fv_tm e -> x ∉ rty_fv τ -> not_overbasety τ ->
+    wf_ctxrR st (Γ ++ [(x, {1 ~r> v2} (mk_op_ret op ^r^ v1))]) ->
+    (⅋{st}⟦[v:fst_ty_of_op op|n1|d1|ϕ1]⟧{Γ}) v1 ->
+    (⅋{st}⟦[v:fst_ty_of_op op|n2|d2|ϕ2]⟧{Γ}) v2 ->
+    (⅋{st}⟦τ⟧{Γ ++ [(x, {1 ~r> v2} (mk_op_ret op ^r^ v1))] }) (e ^t^ x) ->
+    ⅋{st}⟦τ⟧{Γ ++ [(x, {1 ~r> v2} (mk_op_ret op ^r^ v1))] } (tletbiop op v1 v2 e).
+Proof.
+  induction Γ; intros; RD_simp2.
+  - mydestr. inv_rd_simpl1. constructor; auto.
+    + denotation_simp. assert ([] ⊢t tletbiop op v1 v2 e ⋮t ⌊τ⌋). eapply tletbiop_typable; refinement_solver.
+      basic_typing_solver.
+    + exists (eval_op_under_bound_tm op v1 v2). split. apply rR_eval_op_under_bound_tm.
+      intros. assert (x1 ↪* v_x) as Hz by (eapply rR_eval_op_under_bound_tm_min; eauto).
+      auto_under v_x. RD_simp2. simpl.
+      rewrite subst_fresh_tm; auto. rewrite open_subst_same_tm in H10; auto.
+      eapply termR_perserve_rR; refinement_solver.
+      eapply letapp_eval_op_under_bound_tm_termR; eauto; refinement_solver.
+  - constructor; auto. denotation_simp. apply tletbiop_typable_ctx_dummy_cons; auto.
+    intros. auto_under c_x. simpl. eapply IHΓ; eauto.
+    + rewrite fv_of_subst_tm_closed; refinement_solver.
+    + rewrite <- subst_open_var_tm; auto. denotation_simp. basic_typing_solver.
+  - constructor; auto. denotation_simp. apply tletbiop_typable_ctx_dummy_cons; auto.
+    mydestr. auto_meet_exists Hmeet. auto_meet_reduce. auto_under v_x. eapply IHΓ; eauto; fold tm_subst.
+    + rewrite fv_of_subst_tm_closed; refinement_solver.
+    + rewrite <- subst_open_var_tm; auto. denotation_simp. basic_typing_solver. op_solver1.
+  - constructor; auto. denotation_simp. apply tletbiop_typable_ctx_dummy_cons; auto.
+    intros. auto_under v_x. eapply IHΓ; eauto; fold tm_subst.
+    + rewrite fv_of_subst_tm_closed; refinement_solver.
+    + rewrite <- subst_open_var_tm; auto. denotation_simp. basic_typing_solver. refinement_solver.
+Qed.
